src/MicroSail/Symbolic/Sound.v
@@ -72,6 +72,9 @@ Module Soundness
 
     Import DynMutV1.
 
+    Definition inconsistent {Σ} (pc : PathCondition Σ) : Prop :=
+      forall ι, ~ inst ι pc.
+
     Global Instance inst_heap : Inst SymbolicHeap SCHeap :=
       instantiate_list.
     Global Instance instlaws_heap : InstLaws SymbolicHeap SCHeap.
@@ -146,30 +149,53 @@ Module Soundness
       - now f_equal.
     Qed.
 
-    Definition ResultProperty Γ A Σ :=
-      DynamicMutatorResult Γ A Σ -> Prop.
-
     (* UNUSED *)
     Definition syngeq {AT} `{Subst AT, Rewrite AT} {Σ0 Σ1} (ζ1 : Sub Σ0 Σ1) (pc1 : PathCondition Σ1) (a0 : AT Σ0) (a1 : AT Σ1) : Prop :=
       rewrite pc1 a1 (subst ζ1 a0).
 
+    (* A generic preorder on symbolic data. The terms a0 and a1 should be
+       considered to be outputs of the executor along the same path, just with
+       different constraints. More specifically: if we run a symbolic
+       computation up to some point with result a0, then a1 denotes the result if
+       we ran it with the new constraints given by pc1. *)
+    Definition geq {AT A} `{Inst AT A} {Σ0 Σ1} (ζ1 : Sub Σ0 Σ1) (pc1 : PathCondition Σ1) (a0 : AT Σ0) (a1 : AT Σ1) : Prop :=
+      forall (ι0 : SymInstance Σ0) (ι1 : SymInstance Σ1),
+        syminstance_rel ζ1 ι0 ι1 ->
+        (inst ι1 pc1 : Prop) ->
+        inst ι0 a0 = inst ι1 a1.
+
+    (* A preorder on path conditions. This encodes that either pc1 belongs to a
+       longer symbolic execution path or that it's the same path, but with
+       potentially additional constraints. *)
     Definition geqpc {Σ0 Σ1} (ζ1 : Sub Σ0 Σ1) (pc0 : PathCondition Σ0) (pc1 : PathCondition Σ1) : Prop :=
       forall (ι0 : SymInstance Σ0) (ι1 : SymInstance Σ1),
         syminstance_rel ζ1 ι0 ι1 ->
         (inst ι1 pc1 : Prop) ->
         (inst ι0 pc0 : Prop).
 
-    Lemma geqpc_refl {Σ} (pc : PathCondition Σ) :
-      geqpc (sub_id Σ) pc pc.
-    Proof. intros ? ι <-. now rewrite inst_sub_id. Qed.
+    Lemma geq_refl {AT A} `{Inst AT A} {Σ} (pc : PathCondition Σ) (a : AT Σ) :
+      geq (sub_id _) pc a a.
+    Proof. intros ? ? <-. now rewrite inst_sub_id. Qed.
 
-    Definition geq {AT} `{Inst AT} {Σ0 Σ1} (ζ1 : Sub Σ0 Σ1) (pc1 : PathCondition Σ1) (a0 : AT Σ0) (a1 : AT Σ1) : Prop :=
-      forall (ι0 : SymInstance Σ0) (ι1 : SymInstance Σ1),
-        syminstance_rel ζ1 ι0 ι1 ->
-        (inst ι1 pc1 : Prop) ->
-        inst ι0 a0 = inst ι1 a1.
+    Lemma geq_trans {AT A} `{Inst AT A} {Σ1 Σ2 Σ3}
+          {ζ12 : Sub Σ1 Σ2} (pc2 : PathCondition Σ2)
+          {ζ23 : Sub Σ2 Σ3} {pc3 : PathCondition Σ3}
+          {a1 : AT Σ1} (a2 : AT Σ2) {a3 : AT Σ3} :
+      geqpc ζ23 pc2 pc3 ->
+      geq ζ12 pc2 a1 a2 ->
+      geq ζ23 pc3 a2 a3 ->
+      geq (sub_comp ζ12 ζ23) pc3 a1 a3.
+    Proof.
+      intros Hpc23 Ha12 Ha23 ι1 ι3 rel13 Hpc3.
+      pose (inst ι3 ζ23) as ι2.
+      pose proof (Hpc23 ι2 ι3 eq_refl Hpc3) as Hpc2.
+      specialize (Ha23 ι2 ι3 eq_refl Hpc3).
+      apply syminstance_rel_comp in rel13.
+      specialize (Ha12 ι1 ι2 rel13 Hpc2).
+      now transitivity (inst ι2 a2).
+    Qed.
 
-    Lemma geq_subst {AT A} `{InstLaws AT A} {Σ0 Σ1} (ζ1 : Sub Σ0 Σ1) (pc1 : PathCondition Σ1) (a0 : AT Σ0) (a1 : AT Σ1) :
+    Lemma geq_syntactic {AT A} `{InstLaws AT A} {Σ0 Σ1} (ζ1 : Sub Σ0 Σ1) (pc1 : PathCondition Σ1) (a0 : AT Σ0) (a1 : AT Σ1) :
       a1 = subst ζ1 a0 ->
       geq ζ1 pc1 a0 a1.
     Proof.
@@ -177,17 +203,26 @@ Module Soundness
       intros -> * <-. now rewrite inst_subst.
     Qed.
 
-    Lemma geq_refl {AT} `{Inst AT} {Σ} (pc : PathCondition Σ) (a : AT Σ) :
-      geq (sub_id _) pc a a.
-    Proof. intros ? ? <-. now rewrite inst_sub_id. Qed.
+    Lemma geq_subst {AT A} `{InstLaws AT A} {Σ2 Σ3 Σ4} (a : AT Σ2) (ζ23 : Sub Σ2 Σ3) (ζ24 : Sub Σ2 Σ4) (ζ34 : Sub Σ3 Σ4)
+          (pc4 : PathCondition Σ4) :
+      geq ζ34 pc4 ζ23 ζ24 -> geq ζ34 pc4 (subst ζ23 a) (subst ζ24 a).
+    Proof.
+      intros Hζ34 ι3 ι4 rel34 Hpc4. specialize (Hζ34 ι3 ι4 rel34 Hpc4).
+      rewrite ?inst_subst. now f_equal.
+    Qed.
 
     Lemma geq_pre_comp {Σ1 Σ2 Σ3 Σ4} (ζ12 : Sub Σ1 Σ2) (ζ23 : Sub Σ2 Σ3) (ζ24 : Sub Σ2 Σ4) (ζ34 : Sub Σ3 Σ4)
           (pc4 : PathCondition Σ4) :
       geq ζ34 pc4 ζ23 ζ24 -> geq ζ34 pc4 (sub_comp ζ12 ζ23) (sub_comp ζ12 ζ24).
-    Proof.
-      intros H ι3 ι4 rel34 Hpc4. specialize (H ι3 ι4 rel34 Hpc4).
-      unfold sub_comp. rewrite ?inst_subst. now f_equal.
-    Qed.
+    Proof. apply geq_subst. Qed.
+
+    Lemma geq_sub_comp {Σ1 Σ2 Σ3} (pc3 : PathCondition Σ3) (ζ12 : Sub Σ1 Σ2) (ζ23 : Sub Σ2 Σ3) :
+      geq ζ23 pc3 ζ12 (sub_comp ζ12 ζ23).
+    Proof. apply geq_syntactic. reflexivity. Qed.
+
+    Lemma geqpc_refl {Σ} (pc : PathCondition Σ) :
+      geqpc (sub_id Σ) pc pc.
+    Proof. intros ? ι <-. now rewrite inst_sub_id. Qed.
 
     Lemma geqpc_trans {Σ0 Σ1 Σ2} (ζ01 : Sub Σ0 Σ1) (ζ02 : Sub Σ0 Σ2) (ζ12 : Sub Σ1 Σ2)
           (pc0 : PathCondition Σ0) (pc1 : PathCondition Σ1) (pc2 : PathCondition Σ2) :
@@ -199,17 +234,19 @@ Module Soundness
       eauto.
     Qed.
 
-    Definition dmutres_geq_syn {Γ A Σ} `{Subst A} (r1 r2 : DynamicMutatorResult Γ A Σ) : Prop :=
+    (* A proper preorder on the result of a symbolic execution, using the
+    generic geq on every component. *)
+    Definition dmutres_geq {Γ AT A Σ} {instA : Inst AT A} (r1 r2 : DynamicMutatorResult Γ AT Σ) : Prop :=
       match r1 , r2 with
       | MkDynMutResult ζ1 pc1 a1 s1, MkDynMutResult ζ2 pc2 a2 s2 =>
         exists ζ12,
-        ζ2  = sub_comp ζ1 ζ12 /\
-        pc2 = subst ζ12 pc1 /\
-        a2  = subst ζ12 a1 /\
-        s2  = subst ζ12 s1
+        geqpc ζ12 pc1 pc2 /\
+        geq ζ12 pc2 ζ1 ζ2 /\
+        geq ζ12 pc2 a1 a2 /\
+        geq ζ12 pc2 s1 s2
       end.
 
-    Definition dmutres_geq_sem {Γ A V Σ} {instA : Inst A V} (r1 r2 : DynamicMutatorResult Γ A Σ) : Prop :=
+    Definition dmutres_geq_low_level {Γ A V Σ} {instA : Inst A V} (r1 r2 : DynamicMutatorResult Γ A Σ) : Prop :=
       match r1 , r2 with
       | MkDynMutResult ζ1 pc1 a1 s1, MkDynMutResult ζ2 pc2 a2 s2 =>
         exists ζ12,
@@ -222,132 +259,355 @@ Module Soundness
           inst ι1 s1 = inst ι2 s2
       end.
 
-    Lemma dmutres_geq_syn_sem {Γ A V Σ} `{InstLaws A V} :
-      forall r1 r2 : DynamicMutatorResult Γ A Σ,
-        dmutres_geq_syn r1 r2 ->
-        dmutres_geq_sem r1 r2.
+    Lemma dmutres_geq_low_equiv {Γ A V Σ} {instA : Inst A V} :
+      forall (r1 r2 : DynamicMutatorResult Γ A Σ),
+        dmutres_geq r1 r2 <-> dmutres_geq_low_level r1 r2.
     Proof.
-      intros [Σ1 ζ1 pc1 a1 s1] [Σ2 ζ2 pc2 a2 s2] [ζ12 Hgeq]; cbn;
+      intros [Σ1 ζ1 pc1 a1 s1] [Σ2 ζ2 pc2 a2 s2]; cbn. unfold geqpc, geq.
+      split; intros [ζ12 Hgeq]; exists ζ12; intuition.
+    Qed.
+
+    (* A frequent special case. *)
+    Lemma dmutres_geq_syntactic {Γ A V Σ} `{InstLaws A V} :
+      forall r1 r2 : DynamicMutatorResult Γ A Σ,
+        (match r1 , r2 with
+         | MkDynMutResult ζ1 pc1 a1 s1, MkDynMutResult ζ2 pc2 a2 s2 =>
+           exists ζ12,
+           ζ2  = sub_comp ζ1 ζ12 /\
+           pc2 = subst ζ12 pc1 /\
+           a2  = subst ζ12 a1 /\
+           s2  = subst ζ12 s1
+         end
+        ) ->
+        dmutres_geq r1 r2.
+    Proof.
+      intros [Σ1 ζ1 pc1 a1 s1] [Σ2 ζ2 pc2 a2 s2] [ζ12 Hgeq]; cbn - [dmutres_geq];
         destruct_conjs; subst.
+      apply dmutres_geq_low_equiv.
       exists ζ12. intros ? ? <-.
       unfold sub_comp; now rewrite ?inst_subst.
     Qed.
 
-    Definition dmutres_geq_sem' {Γ A V Σ} {instA : Inst A V} (r1 r2 : DynamicMutatorResult Γ A Σ) : Prop :=
-      match r1 , r2 with
-      | MkDynMutResult ζ1 pc1 a1 s1, MkDynMutResult ζ2 pc2 a2 s2 =>
-        exists ζ12,
-        geqpc ζ12 pc1 pc2 /\
-        geq ζ12 pc2 ζ1 ζ2 /\
-        geq ζ12 pc2 a1 a2 /\
-        geq ζ12 pc2 s1 s2
-      end.
-
-    Lemma dmutres_geq_sem_sem' {Γ A V Σ} {instA : Inst A V} :
-      forall (r1 r2 : DynamicMutatorResult Γ A Σ),
-        dmutres_geq_sem r1 r2 <-> dmutres_geq_sem' r1 r2.
-    Proof.
-      intros [Σ1 ζ1 pc1 a1 s1] [Σ2 ζ2 pc2 a2 s2]; cbn.
-      unfold geqpc, geq.
-      split; intros [ζ12 Hgeq]; exists ζ12; intuition.
-    Qed.
-
-    Global Instance dmutres_geq_sem_preorder {Γ A V Σ} `{instLA : InstLaws A V} : PreOrder (@dmutres_geq_sem Γ A V Σ _).
+    Global Instance dmutres_geq_preorder {Γ AT A Σ} `{Inst AT A} : PreOrder (@dmutres_geq Γ AT A Σ _).
     Proof.
       constructor.
-      - intros [Σ1 ζ1 pc a1 s]. cbn. exists (sub_id _).
-        intros ? ? <-. now rewrite inst_sub_id.
-      - intros [Σ1 ζ1 pc1 a1 s1] [Σ2 ζ2 pc2 a2 s2] [Σ3 ζ3 pc3 a3 s3]; cbn.
-        intros [ζ12 H12] [ζ23 H23].
-        exists (sub_comp ζ12 ζ23).
-        intros ι1 ι3. pose (inst ι3 ζ23) as ι2.
-        intros rel12%syminstance_rel_comp.
-        specialize (H12 ι1 ι2 rel12).
-        specialize (H23 ι2 ι3 eq_refl).
-        intuition.
+      - intros [Σ1 ζ1 pc a1 s]. exists (sub_id _).
+        repeat split; try apply geq_refl. apply geqpc_refl.
+      - intros [Σ1 ζ1 pc1 a1 s1] [Σ2 ζ2 pc2 a2 s2] [Σ3 ζ3 pc3 a3 s3] [ζ12] [ζ23]; cbn.
+        destruct_conjs. exists (sub_comp ζ12 ζ23).
+        repeat split.
+        + apply geqpc_trans with ζ12 ζ23 pc2; auto using geq_sub_comp.
+        + apply geq_trans with pc2 ζ2; auto.
+        + apply geq_trans with pc2 a2; auto.
+        + apply geq_trans with pc2 s2; auto.
     Qed.
 
-    Lemma dmutres_geq_sem_pre_comp {A AV} {instA : Inst A AV} {Γ Σ1 Σ2 Σ3}
-          (ζ2 : Sub Σ1 Σ2) (a2 : A Σ2) pc2 (s2 : SymbolicState Γ Σ2)
-          (ζ3 : Sub Σ1 Σ3) (a3 : A Σ3) pc3 (s3 : SymbolicState Γ Σ3) :
+    Global Instance dmutres_geq_rewrite {Γ AT A Σ} `{Inst AT A} : RewriteRelation (@dmutres_geq Γ AT A Σ _).
+    Qed.
+
+    Lemma dmutres_geq_pre_comp {AT A} `{Inst AT A} {Γ Σ1 Σ2 Σ3}
+          (ζ2 : Sub Σ1 Σ2) (a2 : AT Σ2) pc2 (s2 : SymbolicState Γ Σ2)
+          (ζ3 : Sub Σ1 Σ3) (a3 : AT Σ3) pc3 (s3 : SymbolicState Γ Σ3) :
       forall Σ0 (ζ1 : Sub Σ0 Σ1),
-        dmutres_geq_sem (MkDynMutResult ζ2 pc2 a2 s2) (MkDynMutResult ζ3 pc3 a3 s3) ->
-        dmutres_geq_sem (MkDynMutResult (sub_comp ζ1 ζ2) pc2 a2 s2) (MkDynMutResult (sub_comp ζ1 ζ3) pc3 a3 s3).
+        dmutres_geq (MkDynMutResult ζ2 pc2 a2 s2) (MkDynMutResult ζ3 pc3 a3 s3) ->
+        dmutres_geq (MkDynMutResult (sub_comp ζ1 ζ2) pc2 a2 s2) (MkDynMutResult (sub_comp ζ1 ζ3) pc3 a3 s3).
     Proof.
-      intros ? ? [ζ23 H]. exists ζ23.
-      intros ? ? Hrel Hpc. specialize (H _ _ Hrel Hpc).
-      unfold sub_comp. rewrite ?inst_subst. intuition.
+      intros ? ?. intros [ζ23]. exists ζ23. destruct_conjs.
+      repeat split; auto using geq_pre_comp.
     Qed.
 
-    Definition resultprop_specialize {Γ A Σ1 Σ2} (ζ : Sub Σ1 Σ2) :
-      ResultProperty Γ A Σ1 -> ResultProperty Γ A Σ2 :=
-      fun p r => p (cosubst_dmutres ζ r).
+    Definition dmutres_equiv {Γ AT A Σ} {instA : Inst AT A} (r1 r2 : DynamicMutatorResult Γ AT Σ) : Prop :=
+      dmutres_geq r1 r2 /\ dmutres_geq r2 r1.
 
-    Definition resultprop_downwards_closed {Γ AT Σ A} `{Inst AT A} (p : ResultProperty Γ AT Σ) : Prop :=
-      forall (r1 r2 : DynamicMutatorResult Γ AT Σ),
-        dmutres_geq_sem r1 r2 -> p r1 -> p r2.
+    Section StateProp.
 
-    Lemma resultprop_specialize_dcl {Γ A AV Σ1 Σ2} `{Inst A AV} (ζ : Sub Σ1 Σ2) (POST : ResultProperty Γ A Σ1) (POST_dcl : resultprop_downwards_closed POST) :
-      resultprop_downwards_closed (resultprop_specialize ζ POST).
-    Proof.
-      unfold resultprop_downwards_closed, resultprop_specialize.
-      intros [Σ3 ζ3 pc3 a3 s3] [Σ4 ζ4 pc4 a4 s4] [ζ34 Hgeq]. destruct_conjs.
-      apply POST_dcl. exists ζ34.
-      intros ι3 ι4 rel34 Hpc4.
-      specialize (Hgeq ι3 ι4 rel34).
-      unfold syminstance_rel in rel34; subst.
-      unfold sub_comp; rewrite ?inst_subst.
-      intuition.
-    Qed.
+      Definition StateProperty Γ A Σ :=
+        forall Σ1, Sub Σ Σ1 -> PathCondition Σ1 -> A Σ1 -> SymbolicState Γ Σ1 -> Prop.
 
-    Lemma resultprop_specialize_id {Γ A Σ} (P : ResultProperty Γ A Σ) :
-      forall r, resultprop_specialize (sub_id _) P r <-> P r.
-    Proof.
-      intros [Σ' ζ pc a s]; unfold resultprop_specialize; cbn.
-      now rewrite sub_comp_id_left.
-    Qed.
+      Definition stateprop_downwards_closed {Γ Σ AT A} `{Inst AT A} (p : StateProperty Γ AT Σ) : Prop :=
+        forall Σ1 (ζ1 : Sub Σ Σ1) pc1 a1 s1 Σ2 (ζ2 : Sub Σ Σ2) pc2 a2 s2,
+          dmutres_geq (MkDynMutResult ζ1 pc1 a1 s1) (MkDynMutResult ζ2 pc2 a2 s2) ->
+          p Σ1 ζ1 pc1 a1 s1 -> p Σ2 ζ2 pc2 a2 s2.
 
-    Lemma resultprop_specialize_comp {Γ A Σ1 Σ2 Σ3} (ζ12 : Sub Σ1 Σ2) (ζ23 : Sub Σ2 Σ3) (P : ResultProperty Γ A Σ1) :
-      forall r,
-        resultprop_specialize (sub_comp ζ12 ζ23) P r <->
-        resultprop_specialize ζ23 (resultprop_specialize ζ12 P) r.
-    Proof.
-      intros [Σ' ζ pc a s]; unfold resultprop_specialize; cbn.
-      now rewrite sub_comp_assoc.
-    Qed.
+      (* The property always holds vacuously on inconsistent paths. *)
+      Definition stateprop_vacuous {Γ AT Σ} (p : StateProperty Γ AT Σ) : Prop :=
+        forall Σ1 (ζ1 : Sub Σ Σ1) pc a1 s1, inconsistent pc -> p Σ1 ζ1 pc a1 s1.
 
-    Definition resultprop_specialize' {Γ A Σ1 Σ2} (ζ : Sub Σ1 Σ2) (pc2 : PathCondition Σ2) :
-      ResultProperty Γ A Σ1 -> ResultProperty Γ A Σ2 :=
-      fun p r => geqpc (dmutres_substitution r) pc2 (dmutres_pathcondition r) /\ p (cosubst_dmutres ζ r).
+      Definition stateprop_impl {Γ A Σ} (P Q : StateProperty Γ A Σ) : Prop :=
+        forall Σ1 (ζ : Sub Σ Σ1) (pc : PathCondition Σ1) (a : A Σ1) (s : SymbolicState Γ Σ1),
+          P Σ1 ζ pc a s -> Q Σ1 ζ pc a s.
 
-    Lemma resultprop_specialize_dcl' {Γ A AV Σ1 Σ2} `{Inst A AV} (ζ12 : Sub Σ1 Σ2) (pc2 : PathCondition Σ2) (POST : ResultProperty Γ A Σ1) (POST_dcl : resultprop_downwards_closed POST) :
-      resultprop_downwards_closed (resultprop_specialize' ζ12 pc2 POST).
-    Proof.
-      unfold resultprop_downwards_closed, resultprop_specialize'.
-      intros [Σ3 ζ23 pc3 a3 s3] [Σ4 ζ24 pc4 a4 s4] [ζ34 (Hpc34 & Hζ34 & Ha34 & Hs34)]%dmutres_geq_sem_sem'; cbn.
-      intros [Hpc23 Hpost].
-      split.
-      - eapply geqpc_trans; eauto.
-      - revert Hpost. apply POST_dcl.
-        apply dmutres_geq_sem_sem'.
-        exists ζ34. intuition.
-        now apply geq_pre_comp.
-    Qed.
+      Definition stateprop_specialize {Γ A Σ1 Σ2} (ζ : Sub Σ1 Σ2) (p: StateProperty Γ A Σ1) :
+        StateProperty Γ A Σ2 := fun Σ3 ζ3 => p Σ3 (sub_comp ζ ζ3).
 
-    Definition StateProperty Γ A Σ :=
-      forall Σ1, Sub Σ Σ1 -> PathCondition Σ1 -> A Σ1 -> SymbolicState Γ Σ1 -> Prop.
+      Definition stateprop_lift {Γ AT A Σ} {instA : Inst AT A} (ι : SymInstance Σ) (POST : A -> SCState Γ -> Prop) :
+        StateProperty Γ AT Σ :=
+        fun Σ1 ζ1 pc1 v1 s1 =>
+          forall ι1,
+            syminstance_rel ζ1 ι ι1 ->
+            (inst ι1 pc1 : Prop) ->
+            POST (inst ι1 v1) (inst ι1 s1).
 
-    Definition stateprop_specialize {Γ A Σ1 Σ2} (ζ : Sub Σ1 Σ2) (p: StateProperty Γ A Σ1) :
-      StateProperty Γ A Σ2 := fun Σ3 ζ3 => p Σ3 (sub_comp ζ ζ3).
+      Lemma stateprop_lift_dcl {Γ AT A Σ1} `{Inst AT A} (ι1 : SymInstance Σ1) (POST : A -> SCState Γ -> Prop) :
+        stateprop_downwards_closed (stateprop_lift ι1 POST).
+      Proof.
+        unfold stateprop_downwards_closed, stateprop_lift.
+        intros Σ2 ζ2 pc2 a2 s2 Σ3 ζ3 pc3 a3 s3.
+        intros [ζ23 Hgeq]%dmutres_geq_low_equiv Hpost.
+        intros ι3 rel13 Hpc3. pose (inst ι3 ζ23) as ι2.
+        specialize (Hgeq ι2 ι3 eq_refl Hpc3).
+        specialize (Hpost ι2). unfold syminstance_rel in *. subst.
+        intuition.
+      Qed.
 
-    Definition stateprop_impl {Γ A Σ} (P Q : StateProperty Γ A Σ) : Prop :=
-      forall Σ1 (ζ : Sub Σ Σ1) (pc : PathCondition Σ1) (a : A Σ1) (s : SymbolicState Γ Σ1),
-        P Σ1 ζ pc a s -> Q Σ1 ζ pc a s.
+      Lemma stateprop_lift_vac {Γ AT A Σ1} `{Inst AT A} (ι1 : SymInstance Σ1) (POST : A -> SCState Γ -> Prop) :
+        stateprop_vacuous (stateprop_lift ι1 POST).
+      Proof. unfold stateprop_vacuous, stateprop_lift. intuition. Qed.
 
-    Definition stateprop_downwards_closed {Γ Σ A AV} `{Inst A AV} (p : StateProperty Γ A Σ) : Prop :=
-      forall Σ1 (ζ1 : Sub Σ Σ1) pc1 a1 s1 Σ2 (ζ2 : Sub Σ Σ2) pc2 a2 s2,
-        dmutres_geq_sem (MkDynMutResult ζ1 pc1 a1 s1) (MkDynMutResult ζ2 pc2 a2 s2) ->
-        p Σ1 ζ1 pc1 a1 s1 -> p Σ2 ζ2 pc2 a2 s2.
+    End StateProp.
+
+    Section ResultProp.
+
+      Definition ResultProperty Γ A Σ :=
+        DynamicMutatorResult Γ A Σ -> Prop.
+
+      Definition resultprop_specialize {Γ A Σ1 Σ2} (ζ : Sub Σ1 Σ2) :
+        ResultProperty Γ A Σ1 -> ResultProperty Γ A Σ2 :=
+        fun p r => p (cosubst_dmutres ζ r).
+
+      Definition resultprop_downwards_closed {Γ AT Σ A} `{Inst AT A} (p : ResultProperty Γ AT Σ) : Prop :=
+        forall (r1 r2 : DynamicMutatorResult Γ AT Σ),
+          dmutres_geq r1 r2 -> p r1 -> p r2.
+
+      Definition resultprop_vacuous {Γ AT Σ A} `{Inst AT A} (p : ResultProperty Γ AT Σ) : Prop :=
+        forall r, inconsistent (dmutres_pathcondition r) -> p r.
+
+      Lemma resultprop_specialize_vac {Γ A AV Σ1 Σ2} `{Inst A AV} (ζ : Sub Σ1 Σ2)
+            (P : ResultProperty Γ A Σ1) (P_vac : resultprop_vacuous P) :
+        resultprop_vacuous (resultprop_specialize ζ P).
+      Proof.
+        intros [Σ3 ζ23 pc3 a3 s3]; unfold resultprop_specialize; cbn.
+        intros HYP. apply P_vac; auto.
+      Qed.
+
+      Lemma resultprop_specialize_dcl {Γ A AV Σ1 Σ2} `{Inst A AV} (ζ : Sub Σ1 Σ2)
+            (POST : ResultProperty Γ A Σ1) (POST_dcl : resultprop_downwards_closed POST) :
+        resultprop_downwards_closed (resultprop_specialize ζ POST).
+      Proof.
+        unfold resultprop_downwards_closed, resultprop_specialize.
+        intros [Σ3 ζ3 pc3 a3 s3] [Σ4 ζ4 pc4 a4 s4] Hgeq; cbn.
+        now apply POST_dcl, dmutres_geq_pre_comp.
+      Qed.
+
+      Lemma resultprop_specialize_id {Γ A Σ} (P : ResultProperty Γ A Σ) :
+        forall r, resultprop_specialize (sub_id _) P r <-> P r.
+      Proof.
+        intros [Σ' ζ pc a s]; unfold resultprop_specialize; cbn.
+        now rewrite sub_comp_id_left.
+      Qed.
+
+      Lemma resultprop_specialize_comp {Γ A Σ1 Σ2 Σ3} (ζ12 : Sub Σ1 Σ2) (ζ23 : Sub Σ2 Σ3) (P : ResultProperty Γ A Σ1) :
+        forall r,
+          resultprop_specialize (sub_comp ζ12 ζ23) P r <->
+          resultprop_specialize ζ23 (resultprop_specialize ζ12 P) r.
+      Proof.
+        intros [Σ' ζ pc a s]; unfold resultprop_specialize; cbn.
+        now rewrite sub_comp_assoc.
+      Qed.
+
+      Definition resultprop_specialize_pc {Γ A Σ1 Σ2} (ζ : Sub Σ1 Σ2) (pc2 : PathCondition Σ2) :
+        ResultProperty Γ A Σ1 -> ResultProperty Γ A Σ2 :=
+        fun p r => geqpc (dmutres_substitution r) pc2 (dmutres_pathcondition r) /\ p (cosubst_dmutres ζ r).
+
+      Lemma resultprop_specialize_pc_dcl {Γ A AV Σ1 Σ2} `{Inst A AV} (ζ12 : Sub Σ1 Σ2) (pc2 : PathCondition Σ2)
+            (POST : ResultProperty Γ A Σ1) (POST_dcl : resultprop_downwards_closed POST) :
+        resultprop_downwards_closed (resultprop_specialize_pc ζ12 pc2 POST).
+      Proof.
+        unfold resultprop_downwards_closed, resultprop_specialize_pc.
+        intros [Σ3 ζ23 pc3 a3 s3] [Σ4 ζ24 pc4 a4 s4]; cbn.
+        intros [ζ34] [Hpc23 Hpost]; destruct_conjs; cbn.
+        split.
+        - apply geqpc_trans with ζ23 ζ34 pc3; auto.
+        - revert Hpost. apply POST_dcl. exists ζ34.
+          repeat split; auto. now apply geq_pre_comp.
+      Qed.
+
+      Lemma resultprop_specialize_pc_vac {Γ A AV Σ1 Σ2} `{Inst A AV} (ζ : Sub Σ1 Σ2) (pc2 : PathCondition Σ2)
+            (P : ResultProperty Γ A Σ1) (P_vac : resultprop_vacuous P) :
+        resultprop_vacuous (resultprop_specialize_pc ζ pc2 P).
+      Proof.
+      Admitted.
+
+      Definition resultprop_lift {Γ AT A Σ1} {instA : Inst AT A} (ι1 : SymInstance Σ1) (POST : A -> SCState Γ -> Prop) :
+        ResultProperty Γ AT Σ1 :=
+        fun dres =>
+          match dres with
+          | MkDynMutResult ζ2 pc2 a2 s2 =>
+            stateprop_lift ι1 POST ζ2 pc2 a2 s2
+          end.
+
+      Definition resultprop_lift_dcl {Γ AT A Σ1} `{InstLaws AT A} (ι1 : SymInstance Σ1) (POST : A -> SCState Γ -> Prop) :
+        resultprop_downwards_closed (resultprop_lift ι1 POST).
+      Proof.
+        unfold resultprop_downwards_closed, resultprop_lift.
+        intros [Σ3 ζ3 pc3 a3 s3] [Σ4 ζ4 pc4 a4 s4].
+        apply stateprop_lift_dcl.
+      Qed.
+
+      Definition resultprop_lift_vac {Γ AT A Σ1} `{InstLaws AT A} (ι1 : SymInstance Σ1) (POST : A -> SCState Γ -> Prop) :
+        resultprop_vacuous (resultprop_lift ι1 POST).
+      Proof.
+        unfold resultprop_vacuous, resultprop_lift, stateprop_lift.
+        intros [Σ2 ζ2 pc2 a2 s2] Hpc2; cbn in *. intuition.
+      Qed.
+
+    End ResultProp.
+
+    Definition DynamicMutatorArrow Γ1 Γ2 A B Σ0 : Type :=
+      forall Σ1, Sub Σ0 Σ1 -> A Σ1 -> DynamicMutator Γ1 Γ2 B Σ1.
+
+    Definition DynamicMutatorArrow' Γ1 Γ2 A B Σ0 : Type :=
+      forall Σ1,
+        Sub Σ0 Σ1 -> A Σ1 -> PathCondition Σ1 ->
+        SymbolicState Γ1 Σ1 -> Outcome (DynamicMutatorResult Γ2 B Σ1).
+
+    Definition dmut_bind' {Γ1 Γ2 Γ3 A B Σ0}
+               (ma : DynamicMutator Γ1 Γ2 A Σ0) (f : DynamicMutatorArrow' Γ2 Γ3 A B Σ0) : DynamicMutator Γ1 Γ3 B Σ0 :=
+      fun (Σ1 : LCtx) (ζ01 : Sub Σ0 Σ1) pc1 (s1 : SymbolicState Γ1 Σ1) =>
+        outcome_bind (ma Σ1 ζ01 pc1 s1) (fun r : DynamicMutatorResult Γ2 A Σ1 =>
+        outcome_bind (f (dmutres_context r) (sub_comp ζ01 (dmutres_substitution r)) (dmutres_result_value r) (dmutres_pathcondition r) (dmutres_result_state r))
+                     (fun r2 : DynamicMutatorResult Γ3 B (dmutres_context r) => outcome_pure (cosubst_dmutres (dmutres_substitution r) r2))).
+
+    Section Vacuous.
+
+      Definition outcome_vac `{Inst AT A} {Γ Σ} (pc : PathCondition Σ) (o : Outcome (DynamicMutatorResult Γ AT Σ)) : Prop :=
+        forall (P : ResultProperty Γ AT Σ) (P_vac : resultprop_vacuous P),
+          inconsistent pc -> outcome_satisfy o P.
+      Local Hint Unfold outcome_satisfy : core.
+      Local Hint Unfold outcome_vac : core.
+
+      Definition dmut_vac `{Inst AT A} {Γ1 Γ2 Σ0} (d : DynamicMutator Γ1 Γ2 AT Σ0) : Prop :=
+        forall Σ1 (ζ01 : Sub Σ0 Σ1) pc1 s1, outcome_vac pc1 (d Σ1 ζ01 pc1 s1).
+      Local Hint Unfold dmut_vac : core.
+
+      (* TODO: It would be great to reformulate this to use the above. *)
+      Definition dmut_arrow_vac `{Inst AT A, Inst BT B} {Γ1 Γ2 Σ0}
+        (f : DynamicMutatorArrow Γ1 Γ2 AT BT Σ0) : Prop :=
+        forall Σ1 (ζ01 : Sub Σ0 Σ1) pc1 (a1 : AT Σ1) s1,
+          outcome_vac pc1 (f Σ1 ζ01 a1 Σ1 (sub_id _) pc1 s1).
+      Local Hint Unfold dmut_arrow_vac : core.
+
+      Definition dmut_arrow_vac' `{Inst AT A, Inst BT B} {Γ1 Γ2 Σ0}
+        (f : DynamicMutatorArrow' Γ1 Γ2 AT BT Σ0) : Prop :=
+        forall Σ1 (ζ01 : Sub Σ0 Σ1) pc1 (a1 : AT Σ1) s1,
+          outcome_vac pc1 (f Σ1 ζ01 a1 pc1 s1).
+      Local Hint Unfold dmut_arrow_vac' : core.
+
+      Lemma dmut_pure_vac `{Subst AT, Inst AT A} {Γ Σ} (a : AT Σ) :
+        dmut_vac (dmut_pure (Γ := Γ) a).
+      Proof. unfold dmut_pure; auto. Qed.
+      Local Hint Resolve dmut_pure_vac : core.
+
+      Lemma dmut_block_vac `{Inst AT A} {Γ1 Γ2 Σ} :
+        dmut_vac (@dmut_block Γ1 Γ2 AT Σ).
+      Proof. unfold dmut_block; auto. Qed.
+      Local Hint Resolve dmut_block_vac : core.
+
+      Lemma dmut_contradiction_vac `{Inst AT A} {D Γ1 Γ2 Σ} func msg data :
+        dmut_vac (@dmut_contradiction Γ1 Γ2 AT Σ D func msg data).
+      Proof. unfold dmut_contradiction; auto. Qed.
+      Local Hint Resolve dmut_contradiction_vac : core.
+
+      Lemma dmut_fail_vac `{Inst AT A} {D Γ1 Γ2 Σ} func msg data :
+        dmut_vac (@dmut_fail Γ1 Γ2 AT Σ D func msg data).
+      Proof.
+        unfold dmut_fail, dmut_vac, outcome_vac; cbn.
+        unfold inconsistent, Error. intros.
+        (* UH OH *)
+      Admitted.
+      Local Hint Resolve dmut_fail_vac : core.
+
+      Lemma dmut_bind_vac' `{Inst AT A, Inst BT B} {Γ1 Γ2 Γ3 Σ0}
+        (d : DynamicMutator Γ1 Γ2 AT Σ0) (vac_d : dmut_vac d)
+        (f : DynamicMutatorArrow' Γ2 Γ3 AT BT Σ0) (vac_f : dmut_arrow_vac' f) :
+        dmut_vac (dmut_bind' d f).
+      Proof. (* LESS IMPORTANT *) Admitted.
+      Local Hint Resolve dmut_bind_vac' : core.
+
+      Lemma dmut_bind_vac `{Inst AT A, Inst BT B} {Γ1 Γ2 Γ3 Σ0}
+        (d : DynamicMutator Γ1 Γ2 AT Σ0) (vac_d : dmut_vac d)
+        (f : DynamicMutatorArrow Γ2 Γ3 AT BT Σ0) (vac_f : dmut_arrow_vac f) :
+        dmut_vac (dmut_bind d f).
+      Proof. (* MORE IMPORTANT *) Admitted.
+      Local Hint Resolve dmut_bind_vac : core.
+
+      Lemma dmut_sub_vac `{Inst AT A} {Γ1 Γ2 Σ0} (d : DynamicMutator Γ1 Γ2 AT Σ0) (vac_d : dmut_vac d) :
+        forall (Σ1 : LCtx) (ζ1 : Sub Σ0 Σ1), dmut_vac (dmut_sub ζ1 d).
+      Proof. unfold dmut_sub; auto. Qed.
+      Local Hint Resolve dmut_sub_vac : core.
+
+      Lemma dmut_bind_right_vac `{Inst AT A, Inst BT B} {Γ1 Γ2 Γ3 Σ0}
+        (d1 : DynamicMutator Γ1 Γ2 AT Σ0) (d2 : DynamicMutator Γ2 Γ3 BT Σ0) (vac_d1 : dmut_vac d1) (vac_d2 : dmut_vac d2) :
+        dmut_vac (dmut_bind_right d1 d2).
+      Proof. unfold dmut_bind_right; eauto. Qed.
+      Local Hint Resolve dmut_bind_right_vac : core.
+
+      Lemma dmut_demonic_binary_vac `{Inst AT A} {Γ1 Γ2 Σ0}
+        (d1 d2 : DynamicMutator Γ1 Γ2 AT Σ0) (vac_d1 : dmut_vac d1) (vac_d2 : dmut_vac d2) :
+        dmut_vac (dmut_demonic_binary d1 d2).
+      Proof. Admitted.
+      Local Hint Resolve dmut_demonic_binary_vac : core.
+
+      Lemma dmut_angelic_binary_vac `{Inst AT A} {Γ1 Γ2 Σ0}
+        (d1 d2 : DynamicMutator Γ1 Γ2 AT Σ0) (vac_d1 : dmut_vac d1) (vac_d2 : dmut_vac d2) :
+        dmut_vac (dmut_angelic_binary d1 d2).
+      Proof. Admitted.
+      Local Hint Resolve dmut_angelic_binary_vac : core.
+
+      Lemma dmut_demonic_finite_vac {AT A} {F : Type} `{Subst AT, Inst AT A, finite.Finite F} {Γ Σ} (k : F -> DynamicMutator Γ Γ AT Σ) :
+        (forall v, dmut_vac (k v)) ->
+        dmut_vac (dmut_demonic_finite F k).
+      Proof. Admitted.
+      Local Hint Resolve dmut_demonic_finite_vac : core.
+
+      Lemma dmut_assume_formula_vac {Γ Σ} (f : Formula Σ) :
+        dmut_vac (@dmut_assume_formula Γ Σ f).
+      Proof. Admitted.
+      Local Hint Resolve dmut_assume_formula_vac : core.
+
+      Lemma dmut_produce_chunk_vac {Γ Σ} (c : Chunk Σ) :
+        dmut_vac (@dmut_produce_chunk Γ Σ c).
+      Proof. Admitted.
+      Local Hint Resolve dmut_produce_chunk_vac : core.
+
+      Lemma dmut_fresh_vac {AT A} `{Inst AT A} {Γ Σ σ x} (d : DynamicMutator Γ Γ AT (Σ ▻ (x :: σ))) (d_vac : dmut_vac d) :
+        dmut_vac (dmut_fresh (x :: σ) d).
+      Proof. Admitted.
+      Local Hint Resolve dmut_fresh_vac : core.
+
+      Lemma dmut_freshtermvar_vac {Γ Σ σ x} :
+        dmut_vac (@dmut_freshtermvar Γ Σ σ x).
+      Proof. unfold dmut_freshtermvar; auto. Qed.
+      Local Hint Resolve dmut_freshtermvar_vac : core.
+
+      Local Hint Extern 5 (outcome_vac _ (dmut_bind_right _ _ _ _ _)) =>
+        apply dmut_bind_right_vac : core.
+
+      Lemma dmut_produce_vac {Γ Σ} (asn : Assertion Σ) :
+        dmut_vac (@dmut_produce Γ Σ asn).
+      Proof.
+        induction asn; cbn [dmut_produce]; unfold dmut_assume_term; eauto.
+        - destruct (term_get_sum s) as [[]|]; eauto 10.
+        - destruct (term_get_pair s) as [[]|]; auto. admit.
+        - destruct (term_get_record s); eauto. admit.
+        - destruct (term_get_union s) as [[]|]; auto.
+      Admitted.
+
+      Lemma dmut_exec_vac {Γ Σ τ} (s : Stm Γ τ) :
+        dmut_vac (@dmut_exec Γ τ Σ s).
+      Proof. Admitted.
+
+    End Vacuous.
 
     Local Notation "[ ι ] x == y" := (inst ι x = inst ι y) (at level 50).
 
@@ -373,18 +633,6 @@ Module Soundness
         reflexivity.
     Qed.
 
-    Lemma try_solve_formula_geq {Σ0 Σ1} (fml0 : Formula Σ0) (fml1 : Formula Σ1) :
-      forall b0 b1,
-        try_solve_formula fml0 = Some b0 ->
-        try_solve_formula fml1 = Some b1 ->
-        forall (ζ1 : Sub Σ0 Σ1) (pc1 : PathCondition Σ1),
-          geq ζ1 pc1 fml0 fml1 ->
-          forall ι,
-            (inst ι pc1 : Prop) ->
-            b0 = b1.
-    Proof.
-    Admitted.
-
     Lemma dmutres_try_assume_eq_geq {Γ Σ0 σ} (pc0 : PathCondition Σ0) (t1 t2 : Term Σ0 σ) (s0 : SymbolicState Γ Σ0) :
       OptionSpec
         (fun '(MkDynMutResult ζ01 pc1 tt s1) =>
@@ -405,7 +653,7 @@ Module Soundness
         rewrite sub_comp_shift_single.
         rewrite subst_sub_id.
         reflexivity.
-      - now apply geq_subst.
+      - now apply geq_syntactic.
     Qed.
 
     Lemma dmutres_try_assume_eq_spec {Γ Σ σ} (pc : PathCondition Σ) (t1 t2 : Term Σ σ) (s__sym : SymbolicState Γ Σ)
@@ -425,7 +673,7 @@ Module Soundness
       apply (@occurs_check_sound _ _ (@OccursCheckTerm _)) in Heqo;
         auto with typeclass_instances. subst t2.
       split.
-      - apply POST_dcl. exists (sub_shift ςInΣ).
+      - apply POST_dcl. apply dmutres_geq_low_equiv. exists (sub_shift ςInΣ).
         intros * <- Hpc. cbn. rewrite inst_pathcondition_cons in Hpc.
         destruct Hpc as [Hfml Hpc]; cbn in Hfml.
         apply inst_single_shift in Hfml.
@@ -437,7 +685,7 @@ Module Soundness
         rewrite Hfml.
         rewrite ?inst_sub_id.
         auto.
-      - apply POST_dcl. exists (sub_single ςInΣ t).
+      - apply POST_dcl. apply dmutres_geq_low_equiv. exists (sub_single ςInΣ t).
         intros * <- Hpc. rewrite inst_pathcondition_cons.
         rewrite inst_sub_id.
         rewrite <- ?inst_subst. cbn.
@@ -446,6 +694,15 @@ Module Soundness
         rewrite sub_comp_shift_single, subst_sub_id.
         auto.
     Qed.
+
+    (* This should subsume the two lemmas above *)
+    Lemma dmutres_try_assume_eq_spec_v2 {Γ Σ0 σ} (pc0 : PathCondition Σ0) (t1 t2 : Term Σ0 σ) (s0 : SymbolicState Γ Σ0) :
+      OptionSpec
+        (dmutres_equiv (MkDynMutResult (sub_id _) (cons (formula_eq t1 t2) pc0) tt s0))
+        True
+        (dmutres_try_assume_eq pc0 t1 t2 s0).
+    Proof.
+    Admitted.
 
     Lemma dmutres_assume_formula_spec {Γ Σ} (pc : PathCondition Σ) (fml : Formula Σ) (s__sym : SymbolicState Γ Σ)
       (POST : ResultProperty Γ Unit Σ) (POST_dcl : resultprop_downwards_closed POST) :
@@ -460,7 +717,7 @@ Module Soundness
       destruct (dmutres_try_assume_eq_spec pc t1 t2 s__sym POST_dcl); auto. clear H.
       destruct (dmutres_try_assume_eq_spec pc t2 t1 s__sym POST_dcl); auto.
       rewrite H.
-      split; apply POST_dcl; exists (sub_id _); intros ? ? <-;
+      split; apply POST_dcl, dmutres_geq_low_equiv; exists (sub_id _); intros ? ? <-;
           rewrite ?inst_pathcondition_cons, ?inst_sub_id; intuition.
     Qed.
 
@@ -489,9 +746,375 @@ Module Soundness
       - apply geq_refl.
     Qed.
 
+    (* Subsumes the two above. *)
+    Lemma dmutres_assume_formula_spec_v2 {Γ Σ0} (pc0 : PathCondition Σ0) (fml0 : Formula Σ0) (s0 : SymbolicState Γ Σ0) :
+      dmutres_equiv (dmutres_assume_formula pc0 fml0 s0) (MkDynMutResult (sub_id _) (cons fml0 pc0) tt s0).
+    Proof.
+    Admitted.
+
     (* These should be kept abstract in the rest of the proof. If you need some
        property, add a lemma above. *)
+    Local Opaque dmutres_try_assume_eq.
     Local Opaque dmutres_assume_formula.
+
+    Section DownwardsClosure.
+
+      Definition dmut_dcl {Γ1 Γ2 AT Σ0 A} `{Inst AT A} (d : DynamicMutator Γ1 Γ2 AT Σ0) : Prop :=
+        forall Σ1 Σ2 (ζ01 : Sub Σ0 Σ1) pc1 (s1 : SymbolicState Γ1 Σ1) (ζ12 : Sub Σ1 Σ2) pc2 s2 ζ02,
+          geqpc ζ12 pc1 pc2 ->
+          geq ζ12 pc2 s1 s2 ->
+          geq ζ12 pc2 ζ01 ζ02 ->
+          forall (P : ResultProperty Γ2 AT Σ1) (P_dcl : resultprop_downwards_closed P) (P_vac : resultprop_vacuous P)
+                 (Q : ResultProperty Γ2 AT Σ2) (PQ : forall r, resultprop_specialize_pc ζ12 pc2 P r -> Q r),
+            outcome_satisfy (d Σ1 ζ01 pc1 s1) P ->
+            outcome_satisfy (d Σ2 ζ02 pc2 s2) Q.
+
+      Definition dmut_dcl' {Γ1 Γ2 AT Σ0 A} `{Inst AT A} (d : DynamicMutator Γ1 Γ2 AT Σ0) : Prop :=
+        forall Σ1 Σ2 (ζ01 : Sub Σ0 Σ1) pc1 (s1 : SymbolicState Γ1 Σ1) (ζ12 : Sub Σ1 Σ2) pc2 s2 ζ02,
+          geqpc ζ12 pc1 pc2 ->
+          geq ζ12 pc2 s1 s2 ->
+          geq ζ12 pc2 ζ01 ζ02 ->
+          forall (P : ResultProperty Γ2 AT Σ1) (P_dcl : resultprop_downwards_closed P) (P_vac : resultprop_vacuous P),
+            outcome_satisfy (d Σ1 ζ01 pc1 s1) P ->
+            outcome_satisfy (d Σ2 ζ02 pc2 s2) (resultprop_specialize_pc ζ12 pc2 P).
+
+      Lemma dmut_dcl_dcl' {Γ1 Γ2 AT Σ0 A} `{Inst AT A} (d : DynamicMutator Γ1 Γ2 AT Σ0) :
+        dmut_dcl d <-> dmut_dcl' d.
+      Proof.
+        split.
+        - unfold dmut_dcl, dmut_dcl'.
+          intros d_dcl * Hpc12 Hs12 Hζ12 P P_dcl P_vac.
+          eapply d_dcl; eauto.
+        - unfold dmut_dcl, dmut_dcl'.
+          intros d_dcl * Hpc12 Hs12 Hζ12 P P_dcl P_vac Q PQ.
+          intros HP. eapply d_dcl in HP; eauto. revert HP.
+          apply outcome_satisfy_monotonic. intros r. apply PQ.
+      Qed.
+
+      Lemma dmut_pure_dcl {Γ AT Σ A} {subA: Subst AT} {sublAT: SubstLaws AT}
+            {instA : Inst AT A} {instlA : InstLaws AT A} (a : AT Σ) :
+        dmut_dcl (dmut_pure (Γ := Γ) a).
+      Proof.
+        apply dmut_dcl_dcl'. unfold dmut_dcl', dmut_pure; cbn.
+        intros * Hpc12 Hs12 Hζ12 P P_dcl P_vac HP.
+        split. cbn. apply geqpc_refl. revert HP.
+        apply P_dcl.
+        exists ζ12. repeat split; auto.
+        - apply geq_syntactic. change (subst ζ12 ?ζ) with (sub_comp ζ ζ12).
+          now rewrite sub_comp_id_right, sub_comp_id_left.
+        - revert Hζ12.
+          unfold geq. intros HYP ι1 ι2 rel12 Hpc2.
+          specialize (HYP ι1 ι2 rel12 Hpc2) .
+          rewrite ?inst_subst. congruence.
+      Qed.
+
+      Lemma dmut_fail_dcl `{Inst AT A} {D Γ1 Γ2 Σ} func msg data :
+        dmut_dcl (@dmut_fail Γ1 Γ2 AT Σ D func msg data).
+      Proof. apply dmut_dcl_dcl'. unfold dmut_dcl', dmut_fail; cbn. intuition. Qed.
+
+      Definition dmut_arrow_dcl' {Γ1 Γ2 AT A BT B Σ0} `{Inst AT A, Inst BT B}
+        (f : DynamicMutatorArrow' Γ1 Γ2 AT BT Σ0) : Prop :=
+        forall Σ1 Σ2 (ζ01 : Sub Σ0 Σ1) (ζ02 : Sub Σ0 Σ2) (ζ12 : Sub Σ1 Σ2) pc1 pc2 (a1 : AT Σ1) (a2 : AT Σ2) s1 s2,
+          geqpc ζ12 pc1 pc2 ->
+          geq ζ12 pc2 s1 s2 ->
+          geq ζ12 pc2 ζ01 ζ02 ->
+          forall (P : ResultProperty Γ2 BT Σ1) (P_dcl : resultprop_downwards_closed P) (P_vac : resultprop_vacuous P)
+            (Q : ResultProperty Γ2 BT Σ2) (PQ : forall r, resultprop_specialize_pc ζ12 pc2 P r -> Q r),
+            outcome_satisfy (f Σ1 ζ01 a1 pc1 s1) P ->
+            outcome_satisfy (f Σ2 ζ02 a2 pc2 s2) Q.
+
+      Lemma dmut_bind_dcl' {AT A BT B} {substB : Subst BT} {instB : Inst BT B} {instA : Inst AT A}
+            {subA : Subst AT} {subLA : SubstLaws AT} {instLA : InstLaws AT A}
+            {Γ1 Γ2 Γ3 Σ0} (d : DynamicMutator Γ1 Γ2 AT Σ0) (d_dcl : dmut_dcl d)
+            (f : DynamicMutatorArrow' Γ2 Γ3 AT BT Σ0)
+            (f_dcl : dmut_arrow_dcl' f)
+            (f_vac : dmut_arrow_vac' f) :
+        dmut_dcl (dmut_bind' d f).
+      Proof.
+        apply dmut_dcl_dcl'. unfold dmut_dcl', dmut_bind'.
+        intros * Hpc12 Hs12 Hζ12 P P_dcl P_vac.
+        rewrite ?outcome_satisfy_bind; cbn.
+        eapply d_dcl; eauto.
+        - clear - f_dcl P P_dcl P_vac.
+          unfold resultprop_downwards_closed.
+          intros [Σ2 ζ12 pc2 a2 s2] [Σ3 ζ13 pc3 a3 s3] [ζ23 (Hpc23 & Hζ23 & ?)]; cbn in *.
+          rewrite ?outcome_satisfy_bind; cbn.
+          destruct_conjs. eapply f_dcl; eauto using geq_pre_comp.
+          now apply resultprop_specialize_dcl.
+          now apply resultprop_specialize_vac.
+          intros [Σ4 ζ34 pc4 b4 s4]; unfold resultprop_specialize_pc; cbn.
+          intros [Hpc34 HP]; revert HP. apply P_dcl.
+          exists (sub_id _).
+          repeat split; try apply geq_refl.
+          apply geqpc_refl. rewrite <- sub_comp_assoc.
+          clear - Hζ23 Hpc34. intros ? ι4 <-. rewrite inst_sub_id.
+          pose (inst ι4 ζ34) as ι3.
+          pose (inst ι3 ζ23) as ι2.
+          specialize (Hζ23 ι2 ι3 eq_refl).
+          specialize (Hpc34 ι3 ι4 eq_refl).
+          unfold sub_comp; rewrite ?inst_subst.
+          intuition.
+        - intros [Σ3 ζ23 pc3 a3 s3]; cbn.
+          rewrite outcome_satisfy_bind; cbn.
+          now apply f_vac, resultprop_specialize_vac.
+        - intros [Σ3 ζ23 pc3 a3 s3]; unfold resultprop_specialize_pc; cbn.
+          rewrite ?outcome_satisfy_bind; cbn.
+          intros [Hpc23 Hpost]; revert Hpost.
+          eapply f_dcl; try apply geq_refl.
+          + apply geqpc_refl.
+          + clear - Hζ12 Hpc23.
+            intros ? ι3 <- Hpc3.
+            rewrite inst_sub_id.
+            pose (inst ι3 ζ23) as ι2.
+            pose (inst ι2 ζ12) as ι1.
+            specialize (Hpc23 ι2 ι3 eq_refl).
+            specialize (Hζ12 ι1 ι2 eq_refl).
+            unfold sub_comp. rewrite ?inst_subst.
+            intuition.
+          + now apply resultprop_specialize_dcl.
+          + now apply resultprop_specialize_vac.
+          + intros [Σ4 ζ34 pc4 b4 s4]; unfold resultprop_specialize_pc; cbn.
+            intros [Hpc34 Hpost]. rewrite sub_comp_id_left, sub_comp_assoc in Hpost.
+            split; cbn; auto. apply geqpc_trans with ζ23 ζ34 pc3; auto.
+            now apply geq_syntactic.
+      Qed.
+
+      Definition dmut_arrow_dcl {Γ1 Γ2 AT A BT B Σ0} `{Inst AT A, Inst BT B}
+                 (f : DynamicMutatorArrow Γ1 Γ2 AT BT Σ0) : Prop :=
+        forall Σ1 Σ2 (ζ01 : Sub Σ0 Σ1) (ζ02 : Sub Σ0 Σ2) (ζ12 : Sub Σ1 Σ2) pc1 pc2 (a1 : AT Σ1) (a2 : AT Σ2) s1 s2,
+          geqpc ζ12 pc1 pc2 ->
+          geq ζ12 pc2 s1 s2 ->
+          geq ζ12 pc2 ζ01 ζ02 ->
+          forall (P : ResultProperty Γ2 BT Σ1) (P_dcl : resultprop_downwards_closed P) (P_vac : resultprop_vacuous P)
+            (Q : ResultProperty Γ2 BT Σ2) (PQ : forall r, resultprop_specialize_pc ζ12 pc2 P r -> Q r),
+            outcome_satisfy (f Σ1 ζ01 a1 Σ1 (sub_id _) pc1 s1) P ->
+            outcome_satisfy (f Σ2 ζ02 a2 Σ2 (sub_id _) pc2 s2) Q.
+
+      Lemma dmut_bind_dcl {AT A BT B} {substB : Subst BT} {instB : Inst BT B} {instA : Inst AT A}
+            {subA : Subst AT} {subLA : SubstLaws AT} {instLA : InstLaws AT A}
+            {Γ1 Γ2 Γ3 Σ0} (d : DynamicMutator Γ1 Γ2 AT Σ0) (d_wf : dmut_dcl d)
+            (f : DynamicMutatorArrow Γ2 Γ3 AT BT Σ0)
+            (f_dcl : dmut_arrow_dcl f)
+            (f_vac : dmut_arrow_vac f) :
+        dmut_dcl (dmut_bind d f).
+      Proof.
+        apply dmut_dcl_dcl'. unfold dmut_dcl', dmut_bind.
+        intros * Hpc12 Hs12 Hζ12 P P_dcl P_vac.
+        rewrite ?outcome_satisfy_bind; cbn.
+        eapply d_wf; eauto.
+        - clear - f_dcl f_vac P P_dcl P_vac.
+          unfold resultprop_downwards_closed.
+          intros [Σ2 ζ12 pc2 a2 s2] [Σ3 ζ13 pc3 a3 s3] [ζ23 (Hpc23 & Hζ23 & ?)]; cbn in *.
+          rewrite ?outcome_satisfy_bind; cbn.
+          destruct_conjs. eapply f_dcl; eauto using geq_pre_comp.
+          + unfold resultprop_downwards_closed.
+            intros [] [] Hgeq; cbn - [dmutres_geq].
+            apply P_dcl. revert Hgeq. apply dmutres_geq_pre_comp.
+          + unfold resultprop_vacuous.
+            intros [] Hpc; cbn in *. now apply P_vac.
+          + intros [Σ4 ζ34 pc4 b4 s4]; unfold resultprop_specialize_pc; cbn.
+            intros [Hpc34 HP]; revert HP. apply P_dcl.
+            exists (sub_id _).
+            repeat split; try apply geq_refl.
+            apply geqpc_refl.
+            clear - Hζ23 Hpc34.
+            intros ? ι4 <-. rewrite inst_sub_id.
+            pose (inst ι4 ζ34) as ι3.
+            pose (inst ι3 ζ23) as ι2.
+            specialize (Hζ23 ι2 ι3 eq_refl).
+            specialize (Hpc34 ι3 ι4 eq_refl).
+            unfold sub_comp; rewrite ?inst_subst.
+            intuition.
+        - intros [Σ3 ζ23 pc3 a3 s3]; cbn.
+          rewrite outcome_satisfy_bind; cbn.
+          apply f_vac.
+          intros [Σ4 ζ34 pc4 a4 s4]; cbn.
+          intros.
+          now apply P_vac.
+        - intros [Σ3 ζ23 pc3 a3 s3]; unfold resultprop_specialize_pc; cbn.
+          rewrite ?outcome_satisfy_bind; cbn.
+          intros [Hpc23 Hpost]; revert Hpost.
+          eapply f_dcl; try apply geq_refl.
+          + apply geqpc_refl.
+          + clear - Hζ12 Hpc23. intros ? ι3 <- Hpc3.
+            rewrite inst_sub_id.
+            pose (inst ι3 ζ23) as ι2.
+            pose (inst ι2 ζ12) as ι1.
+            specialize (Hpc23 ι2 ι3 eq_refl).
+            specialize (Hζ12 ι1 ι2 eq_refl).
+            unfold sub_comp. rewrite ?inst_subst.
+            intuition.
+          + unfold resultprop_downwards_closed.
+            intros [] [] Hgeq; cbn - [dmutres_geq].
+            apply P_dcl. revert Hgeq. apply dmutres_geq_pre_comp.
+          + unfold resultprop_vacuous.
+            intros [] Hpc; cbn in *. now apply P_vac.
+          + intros [Σ4 ζ34 pc4 b4 s4]; unfold resultprop_specialize_pc; cbn.
+            intros [Hpc34 Hpost]. split.
+            apply geqpc_trans with ζ23 ζ34 pc3; auto. now apply geq_syntactic.
+            now rewrite sub_comp_id_left, sub_comp_assoc in Hpost.
+      Qed.
+
+      Lemma dmut_sub_dcl {Γ1 Γ2 AT A Σ0} {instA : Inst AT A} (d : DynamicMutator Γ1 Γ2 AT Σ0) (d_dcl : dmut_dcl d) :
+        forall (Σ1 : LCtx) (ζ1 : Sub Σ0 Σ1), dmut_dcl (dmut_sub ζ1 d).
+      Proof.
+        unfold dmut_dcl, dmut_sub.
+        intros * Hpc12 Hs12 Hζ12 P P_dcl Q PQ.
+        eapply d_dcl; eauto. now apply geq_pre_comp.
+      Qed.
+
+      Lemma dmut_bind_right_dcl `{InstLaws AT A, InstLaws BT B} {Γ1 Γ2 Γ3 Σ0}
+        (d1 : DynamicMutator Γ1 Γ2 AT Σ0) (d2 : DynamicMutator Γ2 Γ3 BT Σ0)
+        (d1_dcl : dmut_dcl d1) (d2_dcl : dmut_dcl d2) (d2_vac : dmut_vac d2) :
+        dmut_dcl (dmut_bind_right d1 d2).
+      Proof.
+        unfold dmut_bind_right.
+        apply dmut_bind_dcl; auto.
+        - unfold dmut_arrow_dcl.
+          intros until Q. intros PQ.
+          unfold dmut_sub; cbn.
+          rewrite ?sub_comp_id_right.
+          eapply d2_dcl; eauto.
+        - unfold dmut_arrow_vac.
+          intros.
+          now apply dmut_sub_vac.
+      Qed.
+
+      Lemma dmut_demonic_binary_dcl {Γ1 Γ2 AT A Σ0} `{Inst AT A} (d1 d2 : DynamicMutator Γ1 Γ2 AT Σ0) (d_wf1 : dmut_dcl d1) (d_wf2 : dmut_dcl d2) :
+        dmut_dcl (dmut_demonic_binary d1 d2).
+      Proof.
+        unfold dmut_dcl, dmut_demonic_binary; cbn.
+        intros * Hpc12 Hs12 Hζ12 P P_dcl P_vac Q PQ [H1 H2].
+        split.
+        - revert PQ H1. apply d_wf1; auto.
+        - revert PQ H2. apply d_wf2; auto.
+      Qed.
+
+      Lemma dmut_angelic_binary_dcl {Γ1 Γ2 AT A Σ0} `{Inst AT A} (d1 d2 : DynamicMutator Γ1 Γ2 AT Σ0) (d1_dcl : dmut_dcl d1) (d2_dcl : dmut_dcl d2) :
+        dmut_dcl (dmut_angelic_binary d1 d2).
+      Proof.
+        unfold dmut_dcl, dmut_angelic_binary. cbn.
+        intros * Hpc12 Hs12 Hζ12 P P_dcl P_vac Q PQ [H1|H1].
+        - left. revert PQ H1. apply d1_dcl; auto.
+        - right. revert PQ H1. apply d2_dcl; auto.
+      Qed.
+
+      Lemma dmut_assume_formula_dcl {Γ Σ} (f : Formula Σ) :
+        dmut_dcl (@dmut_assume_formula Γ Σ f).
+      Proof.
+        apply dmut_dcl_dcl'. unfold dmut_assume_formula, dmut_dcl'.
+        intros * Hpc12 Hs12 Hζ12 P P_dcl P_vac H.
+        remember (dmutres_assume_formula pc2 (subst ζ02 f) s2) as r.
+        destruct (try_solve_formula_spec (subst ζ01 f));
+        destruct (try_solve_formula_spec (subst ζ02 f)); cbn in *.
+        - clear r Heqr. destruct a, a0; cbn in *; auto.
+          + split; cbn. apply geqpc_refl.
+            revert H. apply P_dcl.
+            exists ζ12. rewrite sub_comp_id_right.
+            repeat split; auto. intros ? ? <-; now rewrite inst_sub_id.
+          + apply resultprop_specialize_pc_vac; cbn; auto.
+            intros ι Hpc2. specialize (Hζ12 _ ι eq_refl Hpc2).
+            specialize (H0 (inst ι ζ12)). specialize (H1 ι).
+            rewrite inst_subst in H0. rewrite inst_subst in H1.
+            rewrite Hζ12 in H0. clear - H0 H1. intuition.
+        - clear H1. destruct a; cbn in *; auto.
+          + subst r. pose proof (dmutres_assume_formula_geq pc2 (subst ζ02 f) s2) as Hgeq.
+            destruct (dmutres_assume_formula pc2 (subst ζ02 f) s2) as [Σ3 ζ23 pc3 [] s3]; cbn in *.
+            destruct Hgeq as [Hpc23 Hs23].
+            split; cbn.
+            * intros ι2 ι3 rel23 Hpc3. specialize (Hpc23 ι2 ι3 rel23 Hpc3).
+              rewrite inst_pathcondition_cons in Hpc23. now destruct Hpc23.
+            * revert H. apply P_dcl. apply dmutres_geq_low_equiv. exists (sub_comp ζ12 ζ23).
+              intros ι1 ι3 rel13 Hpc3. rewrite inst_sub_id.
+              apply syminstance_rel_comp in rel13.
+              pose (inst ι3 ζ23) as ι2.
+              specialize (Hpc23 ι2 ι3 eq_refl Hpc3).
+              specialize (Hs23 ι2 ι3 eq_refl Hpc3).
+              rewrite inst_pathcondition_cons in Hpc23. destruct Hpc23 as [Hfml Hpc2].
+              specialize (Hpc12 ι1 ι2 rel13 Hpc2).
+              specialize (Hs12 ι1 ι2 rel13 Hpc2).
+              specialize (Hζ12 ι1 ι2 rel13 Hpc2).
+              unfold sub_comp. rewrite inst_subst.
+              cbn. repeat split; auto.
+              now transitivity (inst ι2 s2).
+          + subst r. pose proof (dmutres_assume_formula_geq pc2 (subst ζ02 f) s2) as Hgeq.
+            destruct (dmutres_assume_formula pc2 (subst ζ02 f) s2) as [Σ3 ζ23 pc3 [] s3]; cbn in *.
+            destruct Hgeq as [Hpc23 Hs23].
+            split; cbn.
+            * intros ι2 ι3 rel23 Hpc3. specialize (Hpc23 ι2 ι3 rel23 Hpc3).
+              rewrite inst_pathcondition_cons in Hpc23. now destruct Hpc23.
+            * clear - H0 Hpc23 Hpc12. admit.
+        - clear H0 r Heqr. destruct a; cbn; auto. split; cbn.
+          apply geqpc_refl. rewrite sub_comp_id_right.
+          apply (dmutres_assume_formula_spec pc1 (subst ζ01 f) s1) in H; auto.
+          revert H. apply P_dcl. apply dmutres_geq_low_equiv.
+          exists ζ12. intros ι1 ι2 <- Hpc2.
+          rewrite inst_pathcondition_cons, inst_sub_id, ?inst_subst; cbn.
+          intuition.
+          specialize (Hζ12 _ ι2 eq_refl Hpc2). rewrite Hζ12.
+          rewrite <- inst_subst. now apply H1.
+        - clear H0 H1. subst r.
+          pose proof (dmutres_assume_formula_geq pc2 (subst ζ02 f) s2) as Hgeq.
+          destruct (dmutres_assume_formula pc2 (subst ζ02 f) s2) as [Σ3 ζ23 pc3 [] s3]; cbn in *.
+          destruct Hgeq as [Hpc23 Hs23].
+          split; cbn.
+          * intros ι2 ι3 rel23 Hpc3. specialize (Hpc23 ι2 ι3 rel23 Hpc3).
+            rewrite inst_pathcondition_cons in Hpc23. now destruct Hpc23.
+          * apply (dmutres_assume_formula_spec pc1 (subst ζ01 f) s1) in H; auto.
+            revert H. apply P_dcl. apply dmutres_geq_low_equiv.
+            exists (sub_comp ζ12 ζ23). intros ι1 ι3 <- Hpc3.
+            rewrite inst_pathcondition_cons, inst_sub_id.
+            unfold sub_comp; rewrite ?inst_subst; cbn.
+            repeat split; auto.
+            admit.
+            admit.
+            admit.
+      Admitted.
+
+      Lemma dmut_produce_chunk_dcl {Γ Σ} (c : Chunk Σ) :
+        dmut_dcl (@dmut_produce_chunk Γ Σ c).
+      Proof. Admitted.
+
+      Lemma dmut_fresh_dcl {AT A} `{Inst AT A} {Γ Σ σ x} (d : DynamicMutator Γ Γ AT (Σ ▻ (x :: σ))) (d_dcl : dmut_dcl d) :
+        dmut_dcl (dmut_fresh (x :: σ) d).
+      Proof. Admitted.
+
+      Lemma dmut_freshtermvar_dcl {Γ Σ σ x} :
+        dmut_dcl (@dmut_freshtermvar Γ Σ σ x).
+      Proof.
+        apply dmut_dcl_dcl'. unfold dmut_dcl', dmut_freshtermvar; cbn - [dmut_fresh].
+        intros * Hpc12 Hs12 Hζ12 P P_dcl P_vac.
+        eapply dmut_fresh_dcl; eauto.
+        apply dmut_pure_dcl.
+      Qed.
+
+      Lemma dmut_produce_dcl {Γ Σ} (asn : Assertion Σ) :
+        dmut_dcl (@dmut_produce Γ Σ asn).
+      Proof.
+        induction asn; cbn [dmut_produce]; unfold dmut_assume_term.
+        - apply dmut_assume_formula_dcl.
+        - apply dmut_produce_chunk_dcl.
+        - apply dmut_demonic_binary_dcl.
+          apply dmut_bind_right_dcl;
+            auto using dmut_assume_formula_dcl, dmut_produce_vac.
+          apply dmut_bind_right_dcl;
+            auto using dmut_assume_formula_dcl, dmut_produce_vac.
+        - admit.
+        - admit.
+        - apply dmut_fail_dcl.
+        - admit.
+        - apply dmut_fail_dcl.
+        - admit.
+        - admit.
+        - apply dmut_bind_right_dcl; auto using dmut_produce_vac.
+        - now apply dmut_fresh_dcl.
+      Admitted.
+
+      Lemma dmut_exec_dcl {Γ Σ τ} (s : Stm Γ τ) :
+        dmut_vac (@dmut_exec Γ τ Σ s).
+      Proof. Admitted.
+
+    End DownwardsClosure.
 
     Definition scmut_wp {Γ1 Γ2 A}
       (m : SCMut Γ1 Γ2 A)
@@ -532,41 +1155,6 @@ Module Soundness
       apply outcome_satisfy_monotonic.
       intros [Σ2 ζ2 pc2 a2 s2]; cbn.
       intuition.
-    Qed.
-
-    Definition stateprop_lift {Γ AT A Σ} {instA : Inst AT A} (ι : SymInstance Σ) (POST : A -> SCState Γ -> Prop) :
-      StateProperty Γ AT Σ :=
-      fun Σ1 ζ1 pc1 v1 s1 =>
-        forall ι1,
-          syminstance_rel ζ1 ι ι1 ->
-          (inst ι1 pc1 : Prop) ->
-          POST (inst ι1 v1) (inst ι1 s1).
-
-    Lemma stateprop_lift_dcl {Γ AT A Σ1} `{InstLaws AT A} (ι1 : SymInstance Σ1) (POST : A -> SCState Γ -> Prop) :
-      stateprop_downwards_closed (stateprop_lift ι1 POST).
-    Proof.
-      unfold stateprop_downwards_closed, stateprop_lift.
-      intros Σ2 ζ2 pc2 a2 s2 Σ3 ζ3 pc3 a3 s3 [ζ23 Hgeq] Hpost ι3 rel13 Hpc3.
-      pose (inst ι3 ζ23) as ι2.
-      specialize (Hgeq ι2 ι3 eq_refl Hpc3).
-      specialize (Hpost ι2). unfold syminstance_rel in *. subst.
-      intuition.
-    Qed.
-
-    Definition resultprop_lift {Γ AT A Σ1} {instA : Inst AT A} (ι1 : SymInstance Σ1) (POST : A -> SCState Γ -> Prop) :
-      ResultProperty Γ AT Σ1 :=
-      fun dres =>
-        match dres with
-        | MkDynMutResult ζ2 pc2 a2 s2 =>
-          stateprop_lift ι1 POST ζ2 pc2 a2 s2
-        end.
-
-    Definition resultprop_lift_dcl {Γ AT A Σ1} `{InstLaws AT A} (ι1 : SymInstance Σ1) (POST : A -> SCState Γ -> Prop) :
-      resultprop_downwards_closed (resultprop_lift ι1 POST).
-    Proof.
-      unfold resultprop_downwards_closed, resultprop_lift.
-      intros [Σ3 ζ3 pc3 a3 s3] [Σ4 ζ4 pc4 a4 s4].
-      apply stateprop_lift_dcl.
     Qed.
 
     Definition APPROX Γ1 Γ2 AT A {instA : Inst AT A} : Type :=
@@ -635,6 +1223,14 @@ Module Soundness
       box approximates ι d s -> box approximates ι1 (dmut_sub ζ1 d) s.
     Proof. intros H. eapply approximates_box_box; eauto. Qed.
 
+    Lemma approximates_fail `{Inst AT A} {D Γ1 Γ2 Σ} func msg data ι s :
+      box approximates ι (@dmut_fail Γ1 Γ2 AT Σ D func msg data) s.
+    Proof. Admitted.
+
+    Lemma approximates_block `{Inst AT A} {Γ1 Γ2 Σ} (ι : SymInstance Σ) :
+      box approximates ι (@dmut_block Γ1 Γ2 AT Σ) (@scmut_block Γ1 Γ2 A).
+    Proof. Admitted.
+
     Lemma scmut_wp_demonic_binary {Γ1 Γ2 A} (sm1 sm2 : SCMut Γ1 Γ2 A) (s__sc : SCState Γ1) (POST : A -> SCState Γ2 -> Prop) :
       scmut_wp (scmut_demonic_binary sm1 sm2) POST s__sc <->
       scmut_wp sm1 POST s__sc /\ scmut_wp sm2 POST s__sc.
@@ -690,7 +1286,7 @@ Module Soundness
         specialize (dwp Σ1 (sub_id Σ1)). cbn in dwp.
         now rewrite ?sub_comp_id_right, ?subst_sub_id in dwp.
       - intros p Σ2 ζ2. cbn. rewrite subst_sub_comp. revert p.
-        apply POST_dcl. apply dmutres_geq_syn_sem.
+        apply POST_dcl. apply dmutres_geq_syntactic.
         exists ζ2.
         rewrite sub_comp_id_right, sub_comp_id_left.
         now rewrite subst_symbolicstate_produce_chunk.
@@ -703,10 +1299,259 @@ Module Soundness
         (scmut_produce_chunk (inst ι c)).
     Proof.
       intros ? ? ? <- ? ? ? Hwp Hpc. cbn.
-      apply dmut_wp_produce_chunk in Hwp; auto using stateprop_lift_dcl.
-      specialize (Hwp ι1). inster Hwp by apply syminstance_rel_refl.
-      specialize (Hwp Hpc). revert Hwp. destruct s__sym as [δ h]; cbn.
-      now rewrite inst_subst.
+      apply dmut_wp_produce_chunk in Hwp.
+      - specialize (Hwp ι1). inster Hwp by apply syminstance_rel_refl.
+        specialize (Hwp Hpc). destruct s__sym as [δ h]; cbn.
+        now rewrite <- inst_subst.
+      - apply stateprop_lift_dcl.
+    Qed.
+
+    Lemma dmut_wp_sub {Γ1 Γ2 A Σ0} (d : DynamicMutator Γ1 Γ2 A Σ0)
+          (POST : StateProperty Γ2 A Σ0) pc (s : SymbolicState Γ1 Σ0) Σ1 (ζ : Sub Σ0 Σ1) :
+        dmut_wp d POST pc s ->
+        dmut_wp (dmut_sub ζ d) (stateprop_specialize ζ POST) (subst ζ pc) (subst ζ s).
+    Proof.
+      unfold dmut_sub, dmut_wp. intros * Hpost *.
+      specialize (Hpost Σ2 (sub_comp ζ ζ1)).
+      rewrite ?subst_sub_comp in Hpost. revert Hpost.
+      apply outcome_satisfy_monotonic. clear. intros [Σ3 ζ3 pc3 a3 s3].
+      unfold stateprop_specialize. now rewrite sub_comp_assoc.
+    Qed.
+
+    Opaque subst.
+    Opaque sub_up1.
+    Opaque sub_snoc.
+    Opaque wk1.
+    Opaque SubstEnv.
+
+    Lemma dmut_wp_bind {AT A BT B} {instA : Inst AT A} {substB : Subst BT} {instB : Inst BT B}
+          {Γ1 Γ2 Γ3 Σ0} (ma : DynamicMutator Γ1 Γ2 AT Σ0)
+          (f : forall Σ', Sub Σ0 Σ' -> AT Σ' -> DynamicMutator Γ2 Γ3 BT Σ')
+          (f_dcl : dmut_arrow_dcl f)
+          (POST : StateProperty Γ3 BT Σ0) (POST_dcl : stateprop_downwards_closed POST) :
+      forall pc (s0 : SymbolicState Γ1 Σ0),
+        dmut_wp (dmut_bind ma f) POST pc s0 <->
+        dmut_wp ma (fun Σ1 ζ1 pc1 a1 => dmut_wp (f Σ1 ζ1 a1) (stateprop_specialize ζ1 POST) pc1) pc s0.
+    Proof.
+      (* unfold DynamicMutator, dmut_bind, dmut_wp, dmut_dcl in *; cbn; intros pc0 s0. *)
+      (* split; intros H Σ1 ζ1; specialize (H Σ1 ζ1). revert H. *)
+      (* - rewrite outcome_satisfy_bind. apply outcome_satisfy_monotonic. *)
+      (*   intros [Σ2 ζ2 pc2 a2 s2] H Σ3 ζ3. revert H. *)
+      (*   rewrite outcome_satisfy_bind. *)
+      (*   eapply f_dcl. *)
+
+      (* OLD: *)
+      (*   apply (f_wf Σ2 (sub_comp ζ1 ζ2) a2 Σ2 Σ3 (sub_id Σ2) ζ3) in H. *)
+      (*   + revert H. rewrite sub_comp_id_left. *)
+      (*     apply outcome_satisfy_monotonic. *)
+      (*     intros [Σ4 ζ4 pc4 b4 s4]. cbn. *)
+      (*     now rewrite <- sub_comp_assoc. *)
+      (*   + clear f_wf H. *)
+      (*     unfold resultprop_downwards_closed. *)
+      (*     intros [Σ4 ζ4 pc4 b4 s4] [Σ5 ζ5 pc5 b5 s5]. cbn - [dmutres_geq]. *)
+      (*     intros Hgeq. apply POST_dcl. rewrite <- ?sub_comp_assoc. *)
+      (*     revert Hgeq. apply dmutres_geq_pre_comp. *)
+      (* - rewrite outcome_satisfy_bind. revert H. *)
+      (*   apply outcome_satisfy_monotonic. *)
+      (*   intros [Σ2 ζ2 pc2 a2 s2] H. specialize (H Σ2 (sub_id _)). *)
+      (*   revert H. rewrite outcome_satisfy_bind, ?subst_sub_id. *)
+      (*   apply outcome_satisfy_monotonic. *)
+      (*   intros [Σ3 ζ3 pc3 b3 s3]. cbn. *)
+      (*   unfold stateprop_specialize. *)
+      (*   now rewrite sub_comp_id_left, sub_comp_assoc. *)
+    Admitted.
+
+    Lemma dmut_wp_sub_bind {AT A BT B} {instA : Inst AT A} {instB : Inst BT B} {subB: Subst BT}
+          {Γ1 Γ2 Γ3 Σ0 Σ1} (ζ1 : Sub Σ0 Σ1)
+          (ma : DynamicMutator Γ1 Γ2 AT Σ0)
+          (f : forall Σ', Sub Σ0 Σ' -> AT Σ' -> DynamicMutator Γ2 Γ3 BT Σ')
+          (f_dcl : dmut_arrow_dcl f)
+          (POST : StateProperty Γ3 BT Σ1) (POST_dcl : stateprop_downwards_closed POST) :
+      forall pc1 s1,
+        dmut_wp (dmut_sub ζ1 (dmut_bind ma f)) POST pc1 s1 <->
+        dmut_wp
+          (dmut_sub ζ1 ma)
+          (fun Σ2 ζ2 pc2 a2 => dmut_wp (f Σ2 (sub_comp ζ1 ζ2) a2) (stateprop_specialize ζ2 POST) pc2)
+          pc1 s1.
+    Proof.
+      (* unfold DynamicMutator, dmut_bind, dmut_sub, dmut_wp, dmut_dcl in *; cbn; intros pc1 s1. *)
+      (* split; intros H Σ2 ζ2; specialize (H Σ2 ζ2). revert H. *)
+      (* - rewrite outcome_satisfy_bind. apply outcome_satisfy_monotonic. *)
+      (*   intros [Σ3 ζ3 pc3 a3 s3] H Σ4 ζ4. revert H. *)
+      (*   rewrite outcome_satisfy_bind. *)
+      (*   eapply f_dcl. *)
+
+      (* OLD: *)
+      (*   apply (f_wf Σ3 (sub_comp (sub_comp ζ1 ζ2) ζ3) a3 Σ3 Σ4 (sub_id Σ3) ζ4) in H. *)
+      (*   + revert H. rewrite sub_comp_id_left, sub_comp_assoc. *)
+      (*     apply outcome_satisfy_monotonic. *)
+      (*     intros [Σ5 ζ5 b5 s5]. cbn. *)
+      (*     now rewrite <- sub_comp_assoc. *)
+      (*   + revert POST_dcl. clear. intros. *)
+      (*     unfold resultprop_downwards_closed. *)
+      (*     intros [Σ4 ζ4 b4 s4] [Σ5 ζ5 b5 s5] Hgeq. *)
+      (*     cbn. apply POST_dcl. rewrite <- ?sub_comp_assoc. *)
+      (*     revert Hgeq. apply dmutres_geq_sem_pre_comp. *)
+      (* - rewrite outcome_satisfy_bind. revert H. *)
+      (*   apply outcome_satisfy_monotonic. *)
+      (*   intros [Σ3 ζ3 a3 s3] H. specialize (H Σ3 (sub_id _)). *)
+      (*   revert H. rewrite outcome_satisfy_bind, subst_sub_id, sub_comp_assoc. *)
+      (*   apply outcome_satisfy_monotonic. *)
+      (*   intros [Σ4 ζ4 b4 s4]. cbn. *)
+      (*   unfold stateprop_specialize. *)
+      (*   now rewrite sub_comp_id_left, sub_comp_assoc. *)
+    Admitted.
+
+    Lemma dmut_wp_fresh {Γ Σ0 AT A x τ} `{Subst AT, Inst AT A}
+          (d : DynamicMutator Γ Γ AT (Σ0 ▻ (x,τ))%ctx) (d_dcl : dmut_dcl d)
+          (POST : StateProperty Γ AT Σ0)
+          (POST_dcl : stateprop_downwards_closed POST)
+          (pc : PathCondition Σ0) (s : SymbolicState Γ Σ0) :
+      dmut_wp (dmut_fresh (x,τ) d) POST pc s <->
+      dmut_wp d (stateprop_specialize sub_wk1 POST) (subst sub_wk1 pc) (subst sub_wk1 s).
+    Proof.
+      (* OLD: *)
+      (* unfold dmut_wp, dmut_fresh; cbn; split; intros HYP ? ?. *)
+      (* - dependent elimination ζ1 as [@env_snoc Σ0 ζ1 _ v]; cbn in v. *)
+      (*   rewrite <- subst_sub_comp, sub_comp_wk1_tail; cbn. *)
+      (*   specialize (HYP Σ1 ζ1). *)
+      (*   rewrite outcome_satisfy_map in HYP; cbn in *. *)
+      (*   apply (@wfd _ Σ1 _ (env_snoc (sub_id _) (_,τ) v)) in HYP; clear wfd. *)
+      (*   + revert HYP. *)
+      (*     change (wk1 (subst ζ1 ?t)) with (subst (sub_wk1 (b:=(x,τ))) (subst ζ1 t)). *)
+      (*     rewrite <- !subst_sub_comp. *)
+      (*     rewrite !sub_comp_wk1_tail. cbn. *)
+      (*     rewrite <- !sub_snoc_comp. *)
+      (*     rewrite !sub_comp_id_right. *)
+      (*     apply outcome_satisfy_monotonic. *)
+      (*     intros [Σ2 ζ2 pc2 a2 s2]. cbn. clear. *)
+      (*     unfold stateprop_specialize. *)
+      (*     rewrite <- (sub_comp_assoc sub_wk1), sub_comp_wk1_tail. cbn. *)
+      (*     rewrite sub_comp_id_left. *)
+      (*     now rewrite <- sub_comp_assoc, sub_comp_wk1_tail. *)
+      (*   + revert POST_dcl. clear. intros. *)
+      (*     unfold resultprop_downwards_closed. *)
+      (*     intros [Σ2 ζ2 pc2 a2 s2] [Σ3 ζ3 pc3 a3 s3] Hgeq. *)
+      (*     cbn. apply POST_dcl. rewrite <- ?sub_comp_assoc. *)
+      (*     revert Hgeq. apply dmutres_geq_pre_comp. *)
+      (* - rewrite outcome_satisfy_map. *)
+      (*   specialize (HYP (Σ1 ▻ (x,τ)) (sub_up1 ζ1)). *)
+      (*   rewrite <- ?subst_sub_comp, ?sub_comp_wk1_comm in HYP. *)
+      (*   change (wk1 (b := (x,τ)) (subst ζ1 ?t)) with (subst (sub_wk1 (b := (x,τ))) (subst ζ1 t)). *)
+      (*   rewrite <- ?subst_sub_comp. revert HYP. *)
+      (*   apply outcome_satisfy_monotonic. *)
+      (*   intros [Σ2 ζ2 pc2 a2 s2]. clear. *)
+      (*   dependent elimination ζ2 as [@env_snoc Σ1 ζ2 _ t]. *)
+      (*   unfold stateprop_specialize. cbn. *)
+      (*   now rewrite <- ?sub_comp_assoc, <- sub_comp_wk1_comm. *)
+    Admitted.
+
+    Lemma dmut_wp_sub_fresh {Γ Σ0 Σ1 AT A x τ} `{Subst AT, Inst AT A}
+          (ζ1 : Sub Σ0 Σ1)
+          (d : DynamicMutator Γ Γ AT (Σ0 ▻ (x,τ))%ctx)
+          (POST : StateProperty Γ AT Σ1)
+          (POST_dcl : stateprop_downwards_closed POST)
+          (pc : PathCondition Σ1)
+          (s : SymbolicState Γ Σ1) (wfd : dmut_dcl d) :
+      dmut_wp (dmut_sub ζ1 (dmut_fresh (x,τ) d)) POST pc s <->
+      dmut_wp (dmut_sub (sub_up1 ζ1) d) (stateprop_specialize sub_wk1 POST) (subst sub_wk1 pc) (subst sub_wk1 s).
+    Proof.
+      (* OLD: *)
+      (* unfold dmut_wp, dmut_sub, dmut_fresh; cbn; split; intros HYP Σ2 ζ2. *)
+      (* - dependent elimination ζ2 as [@env_snoc Σ1 ζ2 _ v]; cbn in v. *)
+      (*   rewrite <- ?subst_sub_comp, ?sub_comp_wk1_tail; cbn. *)
+      (*   specialize (HYP Σ2 ζ2). *)
+      (*   rewrite outcome_satisfy_map in HYP; cbn in *. *)
+      (*   apply (@wfd _ Σ2 _ (env_snoc (sub_id _) (_,τ) v)) in HYP; clear wfd. *)
+      (*   + change (wk1 (subst ζ2 ?t)) with (subst (sub_wk1 (b:=(x,τ))) (subst ζ2 t)) in HYP. *)
+      (*     rewrite <- ?subst_sub_comp, <- ?sub_snoc_comp, ?sub_comp_id_right, ?sub_comp_wk1_tail in HYP. *)
+      (*     cbn in HYP. rewrite sub_comp_id_right in HYP. *)
+      (*     rewrite <- sub_snoc_comp. revert HYP. *)
+      (*     apply outcome_satisfy_monotonic. *)
+      (*     intros [Σ3 ζ3 pc3 a3 s3]. cbn. clear. unfold stateprop_specialize. *)
+      (*     rewrite <- (sub_comp_assoc sub_wk1), sub_comp_wk1_tail. cbn. *)
+      (*     rewrite sub_comp_id_left. *)
+      (*     now rewrite <- sub_comp_assoc, sub_comp_wk1_tail. *)
+      (*   + revert POST_dcl. clear. intros. *)
+      (*     unfold resultprop_downwards_closed. *)
+      (*     intros [Σ3 ζ3 pc3 a3 s3] [Σ4 ζ4 pc4 a4 s4] Hgeq. *)
+      (*     cbn. apply POST_dcl. rewrite <- ?sub_comp_assoc. *)
+      (*     revert Hgeq. apply dmutres_geq_pre_comp. *)
+      (* - rewrite outcome_satisfy_map. *)
+      (*   specialize (HYP (Σ2 ▻ (x,τ)) (sub_up1 ζ2)). *)
+      (*   rewrite <- ?subst_sub_comp, ?sub_comp_wk1_comm in HYP. *)
+      (*   change (wk1 (b := (x,τ)) (subst ζ2 ?t)) with (subst (sub_wk1 (b := (x,τ))) (subst ζ2 t)). *)
+      (*   rewrite ?sub_up_comp, <- ?subst_sub_comp. *)
+      (*   revert HYP. apply outcome_satisfy_monotonic. *)
+      (*   intros [Σ3 ζ3 pc3 a3 s3]. clear. *)
+      (*   dependent elimination ζ3 as [@env_snoc Σ2 ζ3 _ t]. *)
+      (*   unfold stateprop_specialize. cbn. *)
+      (*   now rewrite <- ?sub_comp_assoc, <- sub_comp_wk1_comm. *)
+    Admitted.
+
+    Lemma dmut_bind_sound {Γ1 Γ2 Γ3 Σ0 AT A BT B}
+      `{Subst AT, Inst AT A, InstLaws BT B} (ι0 : SymInstance Σ0)
+      (dma : DynamicMutator Γ1 Γ2 AT Σ0) (dm_dcl : dmut_dcl dma)
+      (sma : SCMut Γ1 Γ2 A)
+      (dmf : forall Σ1, Sub Σ0 Σ1 -> AT Σ1 -> DynamicMutator Γ2 Γ3 BT Σ1)
+      (dmf_dcl : dmut_arrow_dcl dmf)
+      (smf : A -> SCMut Γ2 Γ3 B) :
+      box approximates ι0 dma sma ->
+      (forall Σ1 (ζ1 : Sub Σ0 Σ1) (a1 : AT Σ1) (ι1 : SymInstance Σ1),
+          syminstance_rel ζ1 ι0 ι1 ->
+          box approximates ι1 (dmf Σ1 ζ1 a1) (smf (inst ι1 a1))) ->
+      box approximates ι0 (dmut_bind dma dmf) (scmut_bind sma smf).
+    Proof.
+      intros H__a H__f.
+      intros Σ1 ζ1 ι1 relι1 pc1 s__sym1 POST H__wp Hpc.
+      apply scmut_wp_bind. revert Hpc.
+      apply dmut_wp_sub_bind in H__wp; auto using stateprop_lift_dcl.
+      specialize (H__a Σ1 ζ1 ι1 relι1).
+      apply H__a. revert H__wp. apply dmut_wp_monotonic.
+      intros Σ2 ζ2 pc2 a2 s2 Hwp2 ι2 rel12 Hpc2. revert Hpc2.
+      specialize (H__f Σ2 (sub_comp ζ1 ζ2) a2 ι2).
+      inster H__f by eapply syminstance_rel_trans; eauto.
+      apply approximates_proj in H__f. apply H__f.
+      revert Hwp2. apply dmut_wp_monotonic.
+      intros Σ3 ζ3 pc3 b3 s__sym3 H__post ι3 rel23 Hpc3.
+      apply H__post. apply (syminstance_rel_trans rel12 rel23). assumption.
+    Qed.
+
+    Lemma dmut_bind_right_sound {Γ1 Γ2 Γ3 Σ0 AT A BT B}
+      `{Subst AT, Inst AT A, InstLaws BT B} (ι0 : SymInstance Σ0)
+      (dma : DynamicMutator Γ1 Γ2 AT Σ0) (dm_dcl : dmut_dcl dma) (sma : SCMut Γ1 Γ2 A)
+      (dmb : DynamicMutator Γ2 Γ3 BT Σ0) (dmb_dcl : dmut_dcl dmb) (smb : SCMut Γ2 Γ3 B) :
+      box approximates ι0 dma sma ->
+      box approximates ι0 dmb smb ->
+      box approximates ι0 (dmut_bind_right dma dmb) (scmut_bind_right sma smb).
+    Proof.
+    Admitted.
+
+    Lemma dmut_fresh_sound {Γ Σ ς τ} (ι : SymInstance Σ)
+          (dm : DynamicMutator Γ Γ Unit (Σ ▻ (ς,τ))) (dm_dcl : dmut_dcl dm)
+          (sm : Lit τ -> SCMut Γ Γ unit) :
+      (forall v, box approximates (env_snoc ι _ v) dm (sm v)) ->
+      box approximates ι
+        (dmut_fresh (ς,τ) dm)
+        (scmut_demonic sm).
+    Proof.
+      intros HYP. unfold box, approximates.
+      intros * <- pc1 s1 POST Hwp Hpc.
+      apply scmut_wp_demonic. intros v.
+      specialize (HYP v (Σ1 ▻ (ς,τ)) (sub_up1 ζ1) (env_snoc ι1 (ς,τ) v)).
+      inster HYP by apply syminstance_rel_up; auto.
+      unfold approximates in HYP.
+      specialize (HYP (subst sub_wk1 pc1) (subst (sub_wk1) s1) POST).
+      rewrite ?inst_subst, ?inst_sub_wk1 in HYP. apply HYP; auto.
+      apply dmut_wp_sub_fresh in Hwp; auto.
+      - revert Hwp.
+        apply dmut_wp_monotonic; cbn.
+        unfold stateprop_impl, stateprop_specialize, stateprop_lift.
+        intros ? ζ * Hpost ι0 rel10.
+        dependent elimination ζ as [@env_snoc Σ0 ζ _ t].
+        apply syminstance_rel_snoc in rel10.
+        apply Hpost. now rewrite sub_comp_wk1_tail.
+      - apply stateprop_lift_dcl.
     Qed.
 
     Lemma dmut_assume_formula_sound {Γ Σ} (ι : SymInstance Σ) (fml : Formula Σ) :
@@ -751,688 +1596,7 @@ Module Soundness
           rewrite inst_subst. auto.
     Qed.
 
-    Definition dmut_wf {Γ1 Γ2 AT Σ0 A} `{Inst AT A} (d : DynamicMutator Γ1 Γ2 AT Σ0) : Prop :=
-      forall Σ1 Σ2 (ζ1 : Sub Σ0 Σ1) (ζ2 : Sub Σ1 Σ2) pc1 (s1 : SymbolicState Γ1 Σ1)
-             (POST : ResultProperty Γ2 AT Σ1) (POST_dcl : resultprop_downwards_closed POST),
-        outcome_satisfy (d Σ1 ζ1 pc1 s1) POST ->
-        outcome_satisfy (d Σ2 (sub_comp ζ1 ζ2) (subst ζ2 pc1) (subst ζ2 s1)) (resultprop_specialize ζ2 POST).
-
-    Lemma dmut_wf_pure {Γ AT Σ A} {subA: Subst AT} {sublAT: SubstLaws AT}
-          {instA : Inst AT A} {instlA : InstLaws AT A} (a : AT Σ) :
-      dmut_wf (dmut_pure (Γ := Γ) a).
-    Proof.
-      unfold dmut_wf, resultprop_specialize; cbn; intros.
-      revert H.
-      apply POST_dcl.
-      exists ζ2; cbn. intros ? ? <- Hpc.
-      rewrite inst_sub_id, sub_comp_id_right, subst_sub_comp.
-      rewrite <- ?inst_subst. auto.
-    Qed.
-
-    Lemma dmut_wf_sub {Γ1 Γ2 AT A Σ0} {instA : Inst AT A} (d : DynamicMutator Γ1 Γ2 AT Σ0) (wf_d : dmut_wf d) :
-      forall (Σ1 : LCtx) (ζ1 : Sub Σ0 Σ1), dmut_wf (dmut_sub ζ1 d).
-    Proof.
-      intros Σ1 ζ1 Σ2 Σ3 ζ2 ζ3 pc2 s2 POST POST_dcl. unfold dmut_sub.
-      rewrite <- sub_comp_assoc. now apply wf_d.
-    Qed.
-
-    Lemma dmut_wf_demonic_binary {Γ1 Γ2 AT A Σ0} `{Inst AT A} (d1 d2 : DynamicMutator Γ1 Γ2 AT Σ0) (wf_d1 : dmut_wf d1) (wf_d2 : dmut_wf d2) :
-      dmut_wf (dmut_demonic_binary d1 d2).
-    Proof.
-      unfold dmut_wf, dmut_demonic_binary in *. cbn.
-      intros * POST_dcl [H1 H2].
-      split.
-      - revert H1. now apply wf_d1.
-      - revert H2. now apply wf_d2.
-    Qed.
-
-    Lemma dmut_wf_angelic_binary {Γ1 Γ2 AT A Σ0} `{Inst AT A} (d1 d2 : DynamicMutator Γ1 Γ2 AT Σ0) (wf_d1 : dmut_wf d1) (wf_d2 : dmut_wf d2) :
-      dmut_wf (dmut_angelic_binary d1 d2).
-    Proof.
-      unfold dmut_wf, dmut_angelic_binary in *. cbn.
-      intros * POST_dcl [H1|H1].
-      - left. revert H1. now apply wf_d1.
-      - right. revert H1. now apply wf_d2.
-    Qed.
-
-    Module WfExperiments.
-
-      Definition dmut_wf {Γ1 Γ2 AT Σ0 A} `{Inst AT A} (d : DynamicMutator Γ1 Γ2 AT Σ0) : Prop :=
-        forall Σ1 Σ2 (ζ01 : Sub Σ0 Σ1) pc1 (s1 : SymbolicState Γ1 Σ1) (ζ12 : Sub Σ1 Σ2) pc2 s2 ζ02,
-          geqpc ζ12 pc1 pc2 ->
-          geq ζ12 pc2 s1 s2 ->
-          geq ζ12 pc2 ζ01 ζ02 ->
-          forall (P : ResultProperty Γ2 AT Σ1) (P_dcl : resultprop_downwards_closed P)
-                 (Q : ResultProperty Γ2 AT Σ2) (PQ : forall r, resultprop_specialize' ζ12 pc2 P r -> Q r),
-            outcome_satisfy (d Σ1 ζ01 pc1 s1) P ->
-            outcome_satisfy (d Σ2 ζ02 pc2 s2) Q.
-
-      Definition dmut_wf' {Γ1 Γ2 AT Σ0 A} `{Inst AT A} (d : DynamicMutator Γ1 Γ2 AT Σ0) : Prop :=
-        forall Σ1 Σ2 (ζ01 : Sub Σ0 Σ1) pc1 (s1 : SymbolicState Γ1 Σ1) (ζ12 : Sub Σ1 Σ2) pc2 s2 ζ02,
-          geqpc ζ12 pc1 pc2 ->
-          geq ζ12 pc2 s1 s2 ->
-          geq ζ12 pc2 ζ01 ζ02 ->
-          forall (POST : ResultProperty Γ2 AT Σ1) (POST_dcl : resultprop_downwards_closed POST),
-            outcome_satisfy (d Σ1 ζ01 pc1 s1) POST ->
-            outcome_satisfy (d Σ2 ζ02 pc2 s2) (resultprop_specialize' ζ12 pc2 POST).
-
-      Definition outcome_result_geq {Γ AT A} `{Inst AT A} {Σ1 Σ2} (ζ12 : Sub Σ1 Σ2)
-                 (pc2 : PathCondition Σ2)
-                 (or1 : Outcome (DynamicMutatorResult Γ AT Σ1))
-                 (or2 : Outcome (DynamicMutatorResult Γ AT Σ2)) : Prop :=
-        forall
-          (P : ResultProperty Γ AT _) (P_dcl : resultprop_downwards_closed P)
-          (Q : ResultProperty Γ AT _) (Q_dcl : resultprop_downwards_closed Q)
-          (PQ : forall r, geqpc (dmutres_substitution r) pc2 (dmutres_pathcondition r) -> resultprop_specialize ζ12 P r -> Q r)
-          (QP : forall r, geqpc (dmutres_substitution r) pc2 (dmutres_pathcondition r) -> Q r -> resultprop_specialize ζ12 P r),
-          outcome_satisfy or1 P ->
-          outcome_satisfy or2 Q.
-
-      Definition dmut_wf'' {Γ1 Γ2 AT Σ0 A} `{Inst AT A} (d : DynamicMutator Γ1 Γ2 AT Σ0) : Prop :=
-        forall Σ1 Σ2 (ζ1 : Sub Σ0 Σ1) (ζ2 : Sub Σ0 Σ2) (ζ12 : Sub Σ1 Σ2) pc1 s1 pc2 s2,
-          geqpc ζ12 pc1 pc2 ->
-          geq ζ12 pc2 s1 s2 ->
-          geq ζ12 pc2 ζ1 ζ2 ->
-          outcome_result_geq ζ12 pc2 (d Σ1 ζ1 pc1 s1) (d Σ2 ζ2 pc2 s2).
-
-      Lemma dmut_wf_wf' {Γ1 Γ2 AT Σ0 A} `{Inst AT A} (d : DynamicMutator Γ1 Γ2 AT Σ0) :
-        dmut_wf d <-> dmut_wf' d.
-      Proof.
-        split.
-        - unfold dmut_wf, dmut_wf'.
-          intros d_wf * Hpc12 Hs12 Hζ12 P P_dcl.
-          eapply d_wf; eauto.
-        - unfold dmut_wf, dmut_wf'.
-          intros d_wf * Hpc12 Hs12 Hζ12 P P_dcl Q PQ.
-          intros HP. eapply d_wf in HP; eauto. revert HP.
-          apply outcome_satisfy_monotonic. intros r. apply PQ.
-      Qed.
-
-      Lemma dmut_wf'_wf'' {Γ1 Γ2 AT Σ0 A} `{Inst AT A} (d : DynamicMutator Γ1 Γ2 AT Σ0) :
-        dmut_wf' d <-> dmut_wf'' d.
-      Proof.
-        split.
-        - unfold dmut_wf, dmut_wf', dmut_wf''. intros d_wf.
-          intros * Hpc12 Hs12 Hζ12. unfold outcome_result_geq.
-          intros * P_dcl * Q_dcl PQ QP. intros HYP.
-          eapply d_wf in HYP; eauto.
-          revert HYP. apply outcome_satisfy_monotonic.
-          intros [Σ3 ζ23 pc3 a3 s3]; cbn.
-          intros [Hpc23 HP]. revert HP. now apply PQ.
-        - unfold dmut_wf, dmut_wf', dmut_wf''. intros d_wf.
-          intros * Hpc12 Hs12 Hζ12 POST POST_dcl.
-          eapply d_wf; eauto using resultprop_specialize_dcl'.
-          + unfold resultprop_specialize, resultprop_specialize'.
-            intros []; intuition.
-          + unfold resultprop_specialize, resultprop_specialize'.
-            intros []; intuition.
-      Qed.
-
-      Lemma dmut_wf_pure {Γ AT Σ A} {subA: Subst AT} {sublAT: SubstLaws AT}
-            {instA : Inst AT A} {instlA : InstLaws AT A} (a : AT Σ) :
-        dmut_wf (dmut_pure (Γ := Γ) a).
-      Proof.
-        unfold dmut_wf, dmut_pure; cbn.
-        intros * Hpc12 Hs12 Hζ12 P P_dcl Q PQ.
-        intros HP. apply PQ. split. cbn.
-        apply geqpc_refl. revert HP.
-        apply P_dcl. apply dmutres_geq_sem_sem'.
-        exists ζ12. repeat split; auto.
-        - apply geq_subst.
-          change (subst ζ12 ?ζ) with (sub_comp ζ ζ12).
-          now rewrite sub_comp_id_right, sub_comp_id_left.
-        - revert Hζ12.
-          unfold geq. intros HYP ι1 ι2 rel12 Hpc2.
-          specialize (HYP ι1 ι2 rel12 Hpc2) .
-          rewrite ?inst_subst. congruence.
-      Qed.
-
-      Definition DynamicMutatorArrow' Γ1 Γ2 A B Σ0 : Type :=
-        forall Σ1,
-          Sub Σ0 Σ1 -> A Σ1 -> PathCondition Σ1 ->
-          SymbolicState Γ1 Σ1 -> Outcome (DynamicMutatorResult Γ2 B Σ1).
-
-      Definition dmut_wf_arrow' {Γ1 Γ2 AT A BT B Σ0} `{Inst AT A, Inst BT B}
-        (f : DynamicMutatorArrow' Γ1 Γ2 AT BT Σ0) : Prop :=
-        forall Σ1 Σ2 (ζ01 : Sub Σ0 Σ1) (ζ02 : Sub Σ0 Σ2) (ζ12 : Sub Σ1 Σ2) pc1 pc2 (a1 : AT Σ1) (a2 : AT Σ2) s1 s2,
-          geqpc ζ12 pc1 pc2 ->
-          geq ζ12 pc2 s1 s2 ->
-          geq ζ12 pc2 ζ01 ζ02 ->
-          forall (P : ResultProperty Γ2 BT Σ1) (P_dcl : resultprop_downwards_closed P)
-            (Q : ResultProperty Γ2 BT Σ2) (PQ : forall r, resultprop_specialize' ζ12 pc2 P r -> Q r),
-            outcome_satisfy (f Σ1 ζ01 a1 pc1 s1) P ->
-            outcome_satisfy (f Σ2 ζ02 a2 pc2 s2) Q.
-
-      Definition dmut_bind' {Γ1 Γ2 Γ3 A B Σ0}
-                 (ma : DynamicMutator Γ1 Γ2 A Σ0) (f : DynamicMutatorArrow' Γ2 Γ3 A B Σ0) : DynamicMutator Γ1 Γ3 B Σ0 :=
-        fun (Σ1 : LCtx) (ζ01 : Sub Σ0 Σ1) pc1 (s1 : SymbolicState Γ1 Σ1) =>
-          outcome_bind (ma Σ1 ζ01 pc1 s1) (fun r : DynamicMutatorResult Γ2 A Σ1 =>
-          outcome_bind (f (dmutres_context r) (sub_comp ζ01 (dmutres_substitution r)) (dmutres_result_value r) (dmutres_pathcondition r) (dmutres_result_state r))
-                       (fun r2 : DynamicMutatorResult Γ3 B (dmutres_context r) => outcome_pure (cosubst_dmutres (dmutres_substitution r) r2))).
-
-      Lemma dmut_wf_bind' {AT A BT B} {substB : Subst BT} {instB : Inst BT B} {instA : Inst AT A}
-            {subA : Subst AT} {subLA : SubstLaws AT} {instLA : InstLaws AT A}
-            {Γ1 Γ2 Γ3 Σ0} (d : DynamicMutator Γ1 Γ2 AT Σ0) (wf_d : dmut_wf d)
-            (f : DynamicMutatorArrow' Γ2 Γ3 AT BT Σ0)
-            (f_wf : dmut_wf_arrow' f) :
-        dmut_wf (dmut_bind' d f).
-      Proof.
-        unfold dmut_wf, dmut_bind'.
-        intros * Hpc12 Hs12 Hζ12 P P_dcl Q PQ.
-        rewrite ?outcome_satisfy_bind; cbn.
-        eapply wf_d; eauto.
-        - clear - f_wf P P_dcl.
-          unfold resultprop_downwards_closed.
-          intros [Σ2 ζ12 pc2 a2 s2] [Σ3 ζ13 pc3 a3 s3] [ζ23 (Hpc23 & Hζ23 & ?)]%dmutres_geq_sem_sem'; cbn in *.
-          rewrite ?outcome_satisfy_bind; cbn.
-          destruct_conjs. eapply f_wf; eauto using geq_pre_comp.
-          now apply resultprop_specialize_dcl.
-          intros [Σ4 ζ34 pc4 b4 s4]; unfold resultprop_specialize'; cbn.
-          intros [Hpc34 HP]; revert HP. apply P_dcl.
-          apply dmutres_geq_sem_sem'. exists (sub_id _).
-          repeat split; try apply geq_refl.
-          apply geqpc_refl.
-          clear - Hζ23 Hpc34. intros ? ι4 <-. rewrite inst_sub_id.
-          pose (inst ι4 ζ34) as ι3.
-          pose (inst ι3 ζ23) as ι2.
-          specialize (Hζ23 ι2 ι3 eq_refl).
-          specialize (Hpc34 ι3 ι4 eq_refl).
-          unfold sub_comp; rewrite ?inst_subst.
-          intuition.
-        - intros [Σ3 ζ23 pc3 a3 s3]; unfold resultprop_specialize'; cbn.
-          rewrite ?outcome_satisfy_bind; cbn.
-          intros [Hpc23 Hpost]; revert Hpost.
-          eapply f_wf; try apply geq_refl.
-          + apply geqpc_refl.
-          + clear - Hζ12 Hpc23.
-            intros ? ι3 <- Hpc3.
-            rewrite inst_sub_id.
-            pose (inst ι3 ζ23) as ι2.
-            pose (inst ι2 ζ12) as ι1.
-            specialize (Hpc23 ι2 ι3 eq_refl).
-            specialize (Hζ12 ι1 ι2 eq_refl).
-            unfold sub_comp. rewrite ?inst_subst.
-            intuition.
-          + now apply resultprop_specialize_dcl.
-          + intros [Σ4 ζ34 pc4 b4 s4]; unfold resultprop_specialize'; cbn.
-            intros [Hpc34 Hpost]. rewrite sub_comp_id_left, sub_comp_assoc in Hpost.
-            apply PQ. split; cbn; auto. eapply geqpc_trans; eauto. now apply geq_subst.
-      Qed.
-
-      Definition DynamicMutatorArrow Γ1 Γ2 A B Σ0 : Type :=
-        forall Σ1, Sub Σ0 Σ1 -> A Σ1 -> DynamicMutator Γ1 Γ2 B Σ1.
-
-      Definition dmut_wf_arrow {Γ1 Γ2 AT A BT B Σ0} `{Inst AT A, Inst BT B}
-                 (f : DynamicMutatorArrow Γ1 Γ2 AT BT Σ0) : Prop :=
-        forall Σ1 Σ2 (ζ01 : Sub Σ0 Σ1) (ζ02 : Sub Σ0 Σ2) (ζ12 : Sub Σ1 Σ2) pc1 pc2 (a1 : AT Σ1) (a2 : AT Σ2) s1 s2,
-          geqpc ζ12 pc1 pc2 ->
-          geq ζ12 pc2 s1 s2 ->
-          geq ζ12 pc2 ζ01 ζ02 ->
-          forall (P : ResultProperty Γ2 BT Σ1) (P_dcl : resultprop_downwards_closed P)
-            (Q : ResultProperty Γ2 BT Σ2) (PQ : forall r, resultprop_specialize' ζ12 pc2 P r -> Q r),
-            outcome_satisfy (f Σ1 ζ01 a1 Σ1 (sub_id _) pc1 s1) P ->
-            outcome_satisfy (f Σ2 ζ02 a2 Σ2 (sub_id _) pc2 s2) Q.
-
-      Lemma dmut_wf_bind {AT A BT B} {substB : Subst BT} {instB : Inst BT B} {instA : Inst AT A}
-            {subA : Subst AT} {subLA : SubstLaws AT} {instLA : InstLaws AT A}
-            {Γ1 Γ2 Γ3 Σ0} (d : DynamicMutator Γ1 Γ2 AT Σ0) (wf_d : dmut_wf d)
-            (f : DynamicMutatorArrow Γ2 Γ3 AT BT Σ0)
-            (f_wf : dmut_wf_arrow f) :
-        dmut_wf (dmut_bind d f).
-      Proof.
-        unfold dmut_wf, dmut_bind.
-        intros * Hpc12 Hs12 Hζ12 P P_dcl Q PQ.
-        rewrite ?outcome_satisfy_bind; cbn.
-        eapply wf_d; eauto.
-        - clear - f_wf P P_dcl.
-          unfold resultprop_downwards_closed.
-          intros [Σ2 ζ12 pc2 a2 s2] [Σ3 ζ13 pc3 a3 s3] [ζ23 (Hpc23 & Hζ23 & ?)]%dmutres_geq_sem_sem'; cbn in *.
-          rewrite ?outcome_satisfy_bind; cbn.
-          destruct_conjs. eapply f_wf; eauto using geq_pre_comp.
-          + unfold resultprop_downwards_closed.
-            intros [] [] Hgeq; cbn - [dmutres_geq_sem].
-            apply P_dcl. revert Hgeq. apply dmutres_geq_sem_pre_comp.
-          + intros [Σ4 ζ34 pc4 b4 s4]; unfold resultprop_specialize'; cbn.
-            intros [Hpc34 HP]; revert HP. apply P_dcl.
-            apply dmutres_geq_sem_sem'. exists (sub_id _).
-            repeat split; try apply geq_refl.
-            apply geqpc_refl.
-            clear - Hζ23 Hpc34.
-            intros ? ι4 <-. rewrite inst_sub_id.
-            pose (inst ι4 ζ34) as ι3.
-            pose (inst ι3 ζ23) as ι2.
-            specialize (Hζ23 ι2 ι3 eq_refl).
-            specialize (Hpc34 ι3 ι4 eq_refl).
-            unfold sub_comp; rewrite ?inst_subst.
-            intuition.
-        - intros [Σ3 ζ23 pc3 a3 s3]; unfold resultprop_specialize'; cbn.
-          rewrite ?outcome_satisfy_bind; cbn.
-          intros [Hpc23 Hpost]; revert Hpost.
-          eapply f_wf; try apply geq_refl.
-          + apply geqpc_refl.
-          + clear - Hζ12 Hpc23. intros ? ι3 <- Hpc3.
-            rewrite inst_sub_id.
-            pose (inst ι3 ζ23) as ι2.
-            pose (inst ι2 ζ12) as ι1.
-            specialize (Hpc23 ι2 ι3 eq_refl).
-            specialize (Hζ12 ι1 ι2 eq_refl).
-            unfold sub_comp. rewrite ?inst_subst.
-            intuition.
-          + unfold resultprop_downwards_closed.
-            intros [] [] Hgeq; cbn - [dmutres_geq_sem].
-            apply P_dcl. revert Hgeq. apply dmutres_geq_sem_pre_comp.
-          + intros [Σ4 ζ34 pc4 b4 s4]; unfold resultprop_specialize'; cbn.
-            intros [Hpc34 Hpost]. apply PQ. split; cbn.
-            eapply geqpc_trans; eauto. now apply geq_subst.
-            now rewrite sub_comp_id_left, sub_comp_assoc in Hpost.
-      Qed.
-
-      Lemma dmut_wf_sub {Γ1 Γ2 AT A Σ0} {instA : Inst AT A} (d : DynamicMutator Γ1 Γ2 AT Σ0) (wf_d : dmut_wf d) :
-        forall (Σ1 : LCtx) (ζ1 : Sub Σ0 Σ1), dmut_wf (dmut_sub ζ1 d).
-      Proof.
-        unfold dmut_wf, dmut_sub.
-        intros * Hpc12 Hs12 Hζ12 P P_dcl Q PQ.
-        eapply wf_d; eauto. now apply geq_pre_comp.
-      Qed.
-
-      Lemma dmut_wf_demonic_binary {Γ1 Γ2 AT A Σ0} `{Inst AT A} (d1 d2 : DynamicMutator Γ1 Γ2 AT Σ0) (wf_d1 : dmut_wf d1) (wf_d2 : dmut_wf d2) :
-        dmut_wf (dmut_demonic_binary d1 d2).
-      Proof.
-        unfold dmut_wf, dmut_demonic_binary in *. cbn.
-        intros * Hpc12 Hs12 Hζ12 P P_dcl Q PQ [H1 H2].
-        split.
-        - revert H1. eapply wf_d1; eauto.
-        - revert H2. eapply wf_d2; eauto.
-      Qed.
-
-      Lemma dmut_wf_angelic_binary {Γ1 Γ2 AT A Σ0} `{Inst AT A} (d1 d2 : DynamicMutator Γ1 Γ2 AT Σ0) (wf_d1 : dmut_wf d1) (wf_d2 : dmut_wf d2) :
-        dmut_wf (dmut_angelic_binary d1 d2).
-      Proof.
-        unfold dmut_wf, dmut_angelic_binary in *. cbn.
-        intros * Hpc12 Hs12 Hζ12 P P_dcl Q PQ [H1|H1].
-        - left. revert H1. eapply wf_d1; eauto.
-        - right. revert H1. eapply wf_d2; eauto.
-      Qed.
-
-      Lemma dmut_wf_assume_formula {Γ Σ} (f : Formula Σ) :
-        dmut_wf (@dmut_assume_formula Γ Σ f).
-      Proof.
-        apply dmut_wf_wf'.
-        unfold dmut_assume_formula, dmut_wf'.
-        intros * Hpc12 Hs12 Hζ12 P P_dcl H.
-        remember (dmutres_assume_formula pc2 (subst ζ02 f) s2) as r.
-        destruct (try_solve_formula_spec (subst ζ01 f));
-        destruct (try_solve_formula_spec (subst ζ02 f)); cbn in *.
-        - clear r Heqr. destruct a, a0; cbn in *; auto.
-          + split; cbn. apply geqpc_refl.
-            revert H. apply P_dcl. apply dmutres_geq_sem_sem'.
-            exists ζ12. rewrite sub_comp_id_right.
-            repeat split; auto. intros ? ? <-; now rewrite inst_sub_id.
-          + assert (forall ι, (inst ι pc2 : Prop) -> False).
-            { intros ι Hpc2. specialize (Hζ12 _ ι eq_refl Hpc2).
-              specialize (H0 (inst ι ζ12)). specialize (H1 ι).
-              rewrite inst_subst in H0. rewrite inst_subst in H1.
-              rewrite Hζ12 in H0. clear - H0 H1. intuition.
-            }
-            split; cbn. apply geqpc_refl. clear - H2.
-            admit.
-        - clear H1. destruct a; cbn in *; auto.
-          + subst r. pose proof (dmutres_assume_formula_geq pc2 (subst ζ02 f) s2) as Hgeq.
-            destruct (dmutres_assume_formula pc2 (subst ζ02 f) s2) as [Σ3 ζ23 pc3 [] s3]; cbn in *.
-            destruct Hgeq as [Hpc23 Hs23].
-            split; cbn.
-            * intros ι2 ι3 rel23 Hpc3. specialize (Hpc23 ι2 ι3 rel23 Hpc3).
-              rewrite inst_pathcondition_cons in Hpc23. now destruct Hpc23.
-            * revert H. apply P_dcl. exists (sub_comp ζ12 ζ23).
-              intros ι1 ι3 rel13 Hpc3. rewrite inst_sub_id.
-              apply syminstance_rel_comp in rel13.
-              pose (inst ι3 ζ23) as ι2.
-              specialize (Hpc23 ι2 ι3 eq_refl Hpc3).
-              specialize (Hs23 ι2 ι3 eq_refl Hpc3).
-              rewrite inst_pathcondition_cons in Hpc23. destruct Hpc23 as [Hfml Hpc2].
-              specialize (Hpc12 ι1 ι2 rel13 Hpc2).
-              specialize (Hs12 ι1 ι2 rel13 Hpc2).
-              specialize (Hζ12 ι1 ι2 rel13 Hpc2).
-              unfold sub_comp. rewrite inst_subst.
-              cbn. repeat split; auto.
-              now transitivity (inst ι2 s2).
-          + subst r. pose proof (dmutres_assume_formula_geq pc2 (subst ζ02 f) s2) as Hgeq.
-            destruct (dmutres_assume_formula pc2 (subst ζ02 f) s2) as [Σ3 ζ23 pc3 [] s3]; cbn in *.
-            destruct Hgeq as [Hpc23 Hs23].
-            split; cbn.
-            * intros ι2 ι3 rel23 Hpc3. specialize (Hpc23 ι2 ι3 rel23 Hpc3).
-              rewrite inst_pathcondition_cons in Hpc23. now destruct Hpc23.
-            * clear - H0 Hpc23 Hpc12. admit.
-        - clear H0 r Heqr. destruct a; cbn; auto. split; cbn.
-          apply geqpc_refl. rewrite sub_comp_id_right.
-          apply (dmutres_assume_formula_spec pc1 (subst ζ01 f) s1) in H; auto.
-          revert H. apply P_dcl. exists ζ12. intros ι1 ι2 <- Hpc2.
-          rewrite inst_pathcondition_cons, inst_sub_id, ?inst_subst; cbn.
-          intuition.
-          specialize (Hζ12 _ ι2 eq_refl Hpc2). rewrite Hζ12.
-          rewrite <- inst_subst. now apply H1.
-        - clear H0 H1. subst r.
-          pose proof (dmutres_assume_formula_geq pc2 (subst ζ02 f) s2) as Hgeq.
-          destruct (dmutres_assume_formula pc2 (subst ζ02 f) s2) as [Σ3 ζ23 pc3 [] s3]; cbn in *.
-          destruct Hgeq as [Hpc23 Hs23].
-          split; cbn.
-          * intros ι2 ι3 rel23 Hpc3. specialize (Hpc23 ι2 ι3 rel23 Hpc3).
-            rewrite inst_pathcondition_cons in Hpc23. now destruct Hpc23.
-          * apply (dmutres_assume_formula_spec pc1 (subst ζ01 f) s1) in H; auto.
-            revert H. apply P_dcl. exists (sub_comp ζ12 ζ23). intros ι1 ι3 <- Hpc3.
-            rewrite inst_pathcondition_cons, inst_sub_id.
-            unfold sub_comp; rewrite ?inst_subst; cbn.
-            repeat split; auto.
-            admit.
-            admit.
-            admit.
-      Admitted.
-
-    End WfExperiments.
-
-    Lemma dmut_wp_sub {Γ1 Γ2 A Σ0} (d : DynamicMutator Γ1 Γ2 A Σ0)
-          (POST : StateProperty Γ2 A Σ0) pc (s : SymbolicState Γ1 Σ0) Σ1 (ζ : Sub Σ0 Σ1) :
-        dmut_wp d POST pc s ->
-        dmut_wp (dmut_sub ζ d) (stateprop_specialize ζ POST) (subst ζ pc) (subst ζ s).
-    Proof.
-      unfold dmut_sub, dmut_wp. intros * Hpost *.
-      specialize (Hpost Σ2 (sub_comp ζ ζ1)).
-      rewrite ?subst_sub_comp in Hpost. revert Hpost.
-      apply outcome_satisfy_monotonic. clear. intros [Σ3 ζ3 pc3 a3 s3].
-      unfold stateprop_specialize. now rewrite sub_comp_assoc.
-    Qed.
-
-
-    Lemma dmut_wf_assume_formula {Γ Σ} (f : Formula Σ) :
-      dmut_wf (@dmut_assume_formula Γ Σ f).
-    Proof.
-      unfold dmut_assume_formula, dmut_wf.
-      intros.
-      destruct (try_solve_formula (subst ζ1 f)) eqn:?; cbn in H.
-      - rewrite subst_sub_comp.
-        pose proof (try_solve_formula_subst ζ2 _ Heqo) as ->.
-        revert H. destruct b; cbn; auto.
-        apply POST_dcl, dmutres_geq_syn_sem.
-        exists ζ2. now rewrite sub_comp_id_left, sub_comp_id_right.
-      - destruct (try_solve_formula_spec (subst (sub_comp ζ1 ζ2) f)).
-        + destruct a; cbn; auto.
-          apply dmutres_assume_formula_spec in H; auto. revert H.
-          unfold resultprop_specialize. cbn.
-          apply POST_dcl. exists ζ2.
-          intros ? ? <- Hpc.
-          rewrite inst_pathcondition_cons.
-          rewrite inst_sub_id, sub_comp_id_right.
-          rewrite <- ?inst_subst.
-          rewrite <- subst_sub_comp.
-          intuition.
-        + clear Heqo H0. cbn.
-          apply dmutres_assume_formula_spec in H; auto.
-          apply dmutres_assume_formula_spec.
-          apply resultprop_specialize_dcl; auto.
-          unfold resultprop_specialize; cbn.
-          revert H. rewrite sub_comp_id_right.
-          apply POST_dcl.
-          apply dmutres_geq_syn_sem. exists ζ2.
-          now rewrite sub_comp_id_left, subst_sub_comp.
-    Qed.
-
-    Lemma dmut_wf_produce_chunk {Γ Σ} (c : Chunk Σ) :
-      dmut_wf (@dmut_produce_chunk Γ Σ c).
-    Proof.
-      unfold dmut_wf, dmut_produce_chunk; cbn.
-      intros * POST_dcl. apply POST_dcl.
-      apply dmutres_geq_syn_sem. exists ζ2.
-      rewrite sub_comp_id_left, sub_comp_id_right.
-      rewrite subst_sub_comp.
-      rewrite subst_symbolicstate_produce_chunk.
-      auto.
-    Qed.
-
-    Lemma dmut_wf_produce {Γ Σ} (asn : Assertion Σ) :
-      dmut_wf (@dmut_produce Γ Σ asn).
-    Proof.
-      induction asn; cbn.
-      - apply dmut_wf_assume_formula.
-      - apply dmut_wf_produce_chunk.
-      - apply dmut_wf_demonic_binary.
-        + admit.
-        + admit.
-      - admit.
-      - destruct (term_get_sum s) eqn:?.
-        destruct s0; now apply dmut_wf_sub.
-        apply dmut_wf_demonic_binary.
-        + admit.
-        + admit.
-      - admit.
-      - destruct (term_get_pair s) eqn:?.
-        destruct p; now apply dmut_wf_sub.
-        admit.
-      - admit.
-      - destruct (term_get_record s) eqn:?.
-        now apply dmut_wf_sub.
-        admit.
-      - destruct (term_get_union s) eqn:?.
-        destruct s0. admit.
-        admit.
-      - admit.
-      - admit.
-    Admitted.
-
     Opaque dmut_assume_formula.
-    Opaque subst.
-    Opaque sub_up1.
-    Opaque sub_snoc.
-    Opaque wk1.
-    Opaque SubstEnv.
-
-    Lemma dmut_wp_bind {Γ1 Γ2 Γ3 A BT Σ0 B} {substB : Subst BT} {instB : Inst BT B} (ma : DynamicMutator Γ1 Γ2 A Σ0)
-          (f : forall Σ', Sub Σ0 Σ' -> A Σ' -> DynamicMutator Γ2 Γ3 BT Σ')
-          (f_wf : forall Σ' ζ a, dmut_wf (f Σ' ζ a))
-          (POST : StateProperty Γ3 BT Σ0) (POST_dcl : stateprop_downwards_closed POST) :
-      forall pc (s0 : SymbolicState Γ1 Σ0),
-        dmut_wp (dmut_bind ma f) POST pc s0 <->
-        dmut_wp ma (fun Σ1 ζ1 pc1 a1 => dmut_wp (f Σ1 ζ1 a1) (stateprop_specialize ζ1 POST) pc1) pc s0.
-    Proof.
-      unfold DynamicMutator, dmut_bind, dmut_wp, dmut_wf in *; cbn; intros s0.
-      split; intros H Σ1 ζ1; specialize (H Σ1 ζ1). revert H.
-      - rewrite outcome_satisfy_bind. apply outcome_satisfy_monotonic.
-        intros [Σ2 ζ2 pc2 a2 s2] H Σ3 ζ3.
-        rewrite outcome_satisfy_bind in H.
-        apply (f_wf Σ2 (sub_comp ζ1 ζ2) a2 Σ2 Σ3 (sub_id Σ2) ζ3) in H.
-        + revert H. rewrite sub_comp_id_left.
-          apply outcome_satisfy_monotonic.
-          intros [Σ4 ζ4 pc4 b4 s4]. cbn.
-          now rewrite <- sub_comp_assoc.
-        + clear f_wf H.
-          unfold resultprop_downwards_closed.
-          intros [Σ4 ζ4 pc4 b4 s4] [Σ5 ζ5 pc5 b5 s5]. cbn - [dmutres_geq_sem].
-          intros Hgeq. apply POST_dcl. rewrite <- ?sub_comp_assoc.
-          revert Hgeq. apply dmutres_geq_sem_pre_comp.
-      - rewrite outcome_satisfy_bind. revert H.
-        apply outcome_satisfy_monotonic.
-        intros [Σ2 ζ2 pc2 a2 s2] H. specialize (H Σ2 (sub_id _)).
-        revert H. rewrite outcome_satisfy_bind, ?subst_sub_id.
-        apply outcome_satisfy_monotonic.
-        intros [Σ3 ζ3 pc3 b3 s3]. cbn.
-        unfold stateprop_specialize.
-        now rewrite sub_comp_id_left, sub_comp_assoc.
-    Qed.
-
-    Lemma dmut_wp_sub_bind {A BT B} {subB : Subst BT} {instB : Inst BT B} {Γ1 Γ2 Γ3  Σ0 Σ1} (ζ1 : Sub Σ0 Σ1)
-          (ma : DynamicMutator Γ1 Γ2 A Σ0)
-          (f : forall Σ', Sub Σ0 Σ' -> A Σ' -> DynamicMutator Γ2 Γ3 BT Σ')
-          (f_wf : forall Σ' ζ a, dmut_wf (f Σ' ζ a))
-          (POST : StateProperty Γ3 BT Σ1) (POST_dcl : stateprop_downwards_closed POST) :
-      forall pc1 s1,
-        dmut_wp (dmut_sub ζ1 (dmut_bind ma f)) POST pc1 s1 <->
-        dmut_wp
-          (dmut_sub ζ1 ma)
-          (fun Σ2 ζ2 pc2 a2 => dmut_wp (f Σ2 (sub_comp ζ1 ζ2) a2) (stateprop_specialize ζ2 POST) pc2)
-          pc1 s1.
-    Proof.
-      (* unfold DynamicMutator, dmut_bind, dmut_sub, dmut_wp, dmut_wf in *; cbn; intros s0. *)
-      (* split; intros H Σ2 ζ2; specialize (H Σ2 ζ2). revert H. *)
-      (* - rewrite outcome_satisfy_bind. apply outcome_satisfy_monotonic. *)
-      (*   intros [Σ3 ζ3 a3 s3] H Σ4 ζ4. *)
-      (*   rewrite outcome_satisfy_bind in H. *)
-      (*   apply (f_wf Σ3 (sub_comp (sub_comp ζ1 ζ2) ζ3) a3 Σ3 Σ4 (sub_id Σ3) ζ4) in H. *)
-      (*   + revert H. rewrite sub_comp_id_left, sub_comp_assoc. *)
-      (*     apply outcome_satisfy_monotonic. *)
-      (*     intros [Σ5 ζ5 b5 s5]. cbn. *)
-      (*     now rewrite <- sub_comp_assoc. *)
-      (*   + revert POST_dcl. clear. intros. *)
-      (*     unfold resultprop_downwards_closed. *)
-      (*     intros [Σ4 ζ4 b4 s4] [Σ5 ζ5 b5 s5] Hgeq. *)
-      (*     cbn. apply POST_dcl. rewrite <- ?sub_comp_assoc. *)
-      (*     revert Hgeq. apply dmutres_geq_sem_pre_comp. *)
-      (* - rewrite outcome_satisfy_bind. revert H. *)
-      (*   apply outcome_satisfy_monotonic. *)
-      (*   intros [Σ3 ζ3 a3 s3] H. specialize (H Σ3 (sub_id _)). *)
-      (*   revert H. rewrite outcome_satisfy_bind, subst_sub_id, sub_comp_assoc. *)
-      (*   apply outcome_satisfy_monotonic. *)
-      (*   intros [Σ4 ζ4 b4 s4]. cbn. *)
-      (*   unfold stateprop_specialize. *)
-      (*   now rewrite sub_comp_id_left, sub_comp_assoc. *)
-    Admitted.
-
-    Lemma dmut_wp_fresh {Γ Σ0 AT A x τ} `{Subst AT, Inst AT A}
-          (d : DynamicMutator Γ Γ AT (Σ0 ▻ (x,τ))%ctx) (wfd : dmut_wf d)
-          (POST : StateProperty Γ AT Σ0)
-          (POST_dcl : stateprop_downwards_closed POST)
-          (pc : PathCondition Σ0) (s : SymbolicState Γ Σ0) :
-      dmut_wp (dmut_fresh (x,τ) d) POST pc s <->
-      dmut_wp d (stateprop_specialize sub_wk1 POST) (subst sub_wk1 pc) (subst sub_wk1 s).
-    Proof.
-      unfold dmut_wp, dmut_fresh; cbn; split; intros HYP ? ?.
-      - dependent elimination ζ1 as [@env_snoc Σ0 ζ1 _ v]; cbn in v.
-        rewrite <- subst_sub_comp, sub_comp_wk1_tail; cbn.
-        specialize (HYP Σ1 ζ1).
-        rewrite outcome_satisfy_map in HYP; cbn in *.
-        apply (@wfd _ Σ1 _ (env_snoc (sub_id _) (_,τ) v)) in HYP; clear wfd.
-        + revert HYP.
-          change (wk1 (subst ζ1 ?t)) with (subst (sub_wk1 (b:=(x,τ))) (subst ζ1 t)).
-          rewrite <- !subst_sub_comp.
-          rewrite !sub_comp_wk1_tail. cbn.
-          rewrite <- !sub_snoc_comp.
-          rewrite !sub_comp_id_right.
-          apply outcome_satisfy_monotonic.
-          intros [Σ2 ζ2 pc2 a2 s2]. cbn. clear.
-          unfold stateprop_specialize.
-          rewrite <- (sub_comp_assoc sub_wk1), sub_comp_wk1_tail. cbn.
-          rewrite sub_comp_id_left.
-          now rewrite <- sub_comp_assoc, sub_comp_wk1_tail.
-        + revert POST_dcl. clear. intros.
-          unfold resultprop_downwards_closed.
-          intros [Σ2 ζ2 pc2 a2 s2] [Σ3 ζ3 pc3 a3 s3] Hgeq.
-          cbn. apply POST_dcl. rewrite <- ?sub_comp_assoc.
-          revert Hgeq. apply dmutres_geq_sem_pre_comp.
-      - rewrite outcome_satisfy_map.
-        specialize (HYP (Σ1 ▻ (x,τ)) (sub_up1 ζ1)).
-        rewrite <- ?subst_sub_comp, ?sub_comp_wk1_comm in HYP.
-        change (wk1 (b := (x,τ)) (subst ζ1 ?t)) with (subst (sub_wk1 (b := (x,τ))) (subst ζ1 t)).
-        rewrite <- ?subst_sub_comp. revert HYP.
-        apply outcome_satisfy_monotonic.
-        intros [Σ2 ζ2 pc2 a2 s2]. clear.
-        dependent elimination ζ2 as [@env_snoc Σ1 ζ2 _ t].
-        unfold stateprop_specialize. cbn.
-        now rewrite <- ?sub_comp_assoc, <- sub_comp_wk1_comm.
-    Qed.
-
-    Lemma dmut_wp_sub_fresh {Γ Σ0 Σ1 AT A x τ} `{Subst AT, Inst AT A}
-          (ζ1 : Sub Σ0 Σ1)
-          (d : DynamicMutator Γ Γ AT (Σ0 ▻ (x,τ))%ctx)
-          (POST : StateProperty Γ AT Σ1)
-          (POST_dcl : stateprop_downwards_closed POST)
-          (pc : PathCondition Σ1)
-          (s : SymbolicState Γ Σ1) (wfd : dmut_wf d) :
-      dmut_wp (dmut_sub ζ1 (dmut_fresh (x,τ) d)) POST pc s <->
-      dmut_wp (dmut_sub (sub_up1 ζ1) d) (stateprop_specialize sub_wk1 POST) (subst sub_wk1 pc) (subst sub_wk1 s).
-    Proof.
-      unfold dmut_wp, dmut_sub, dmut_fresh; cbn; split; intros HYP Σ2 ζ2.
-      - dependent elimination ζ2 as [@env_snoc Σ1 ζ2 _ v]; cbn in v.
-        rewrite <- ?subst_sub_comp, ?sub_comp_wk1_tail; cbn.
-        specialize (HYP Σ2 ζ2).
-        rewrite outcome_satisfy_map in HYP; cbn in *.
-        apply (@wfd _ Σ2 _ (env_snoc (sub_id _) (_,τ) v)) in HYP; clear wfd.
-        + change (wk1 (subst ζ2 ?t)) with (subst (sub_wk1 (b:=(x,τ))) (subst ζ2 t)) in HYP.
-          rewrite <- ?subst_sub_comp, <- ?sub_snoc_comp, ?sub_comp_id_right, ?sub_comp_wk1_tail in HYP.
-          cbn in HYP. rewrite sub_comp_id_right in HYP.
-          rewrite <- sub_snoc_comp. revert HYP.
-          apply outcome_satisfy_monotonic.
-          intros [Σ3 ζ3 pc3 a3 s3]. cbn. clear. unfold stateprop_specialize.
-          rewrite <- (sub_comp_assoc sub_wk1), sub_comp_wk1_tail. cbn.
-          rewrite sub_comp_id_left.
-          now rewrite <- sub_comp_assoc, sub_comp_wk1_tail.
-        + revert POST_dcl. clear. intros.
-          unfold resultprop_downwards_closed.
-          intros [Σ3 ζ3 pc3 a3 s3] [Σ4 ζ4 pc4 a4 s4] Hgeq.
-          cbn. apply POST_dcl. rewrite <- ?sub_comp_assoc.
-          revert Hgeq. apply dmutres_geq_sem_pre_comp.
-      - rewrite outcome_satisfy_map.
-        specialize (HYP (Σ2 ▻ (x,τ)) (sub_up1 ζ2)).
-        rewrite <- ?subst_sub_comp, ?sub_comp_wk1_comm in HYP.
-        change (wk1 (b := (x,τ)) (subst ζ2 ?t)) with (subst (sub_wk1 (b := (x,τ))) (subst ζ2 t)).
-        rewrite ?sub_up_comp, <- ?subst_sub_comp.
-        revert HYP. apply outcome_satisfy_monotonic.
-        intros [Σ3 ζ3 pc3 a3 s3]. clear.
-        dependent elimination ζ3 as [@env_snoc Σ2 ζ3 _ t].
-        unfold stateprop_specialize. cbn.
-        now rewrite <- ?sub_comp_assoc, <- sub_comp_wk1_comm.
-    Qed.
-
-    Lemma dmut_bind_sound {Γ1 Γ2 Γ3 Σ0 AT A BT B}
-      `{Subst AT, Inst AT A, InstLaws BT B} (ι0 : SymInstance Σ0)
-      (dma : DynamicMutator Γ1 Γ2 AT Σ0) (wfdm : dmut_wf dma)
-      (sma : SCMut Γ1 Γ2 A)
-      (dmf : forall Σ1, Sub Σ0 Σ1 -> AT Σ1 -> DynamicMutator Γ2 Γ3 BT Σ1)
-      (dmf_wf : forall Σ1 ζ a, dmut_wf (dmf Σ1 ζ a))
-      (smf : A -> SCMut Γ2 Γ3 B) :
-      box approximates ι0 dma sma ->
-      (forall Σ1 (ζ1 : Sub Σ0 Σ1) (a1 : AT Σ1) (ι1 : SymInstance Σ1),
-          syminstance_rel ζ1 ι0 ι1 ->
-          box approximates ι1 (dmf Σ1 ζ1 a1) (smf (inst ι1 a1))) ->
-      box approximates ι0 (dmut_bind dma dmf) (scmut_bind sma smf).
-    Proof.
-      intros H__a H__f.
-      intros Σ1 ζ1 ι1 relι1 pc1 s__sym1 POST H__wp Hpc.
-      apply scmut_wp_bind. revert Hpc.
-      apply dmut_wp_sub_bind in H__wp; auto using stateprop_lift_dcl.
-      specialize (H__a Σ1 ζ1 ι1 relι1).
-      apply H__a. revert H__wp. apply dmut_wp_monotonic.
-      intros Σ2 ζ2 pc2 a2 s2 Hwp2 ι2 rel12 Hpc2. revert Hpc2.
-      specialize (H__f Σ2 (sub_comp ζ1 ζ2) a2 ι2).
-      inster H__f by eapply syminstance_rel_trans; eauto.
-      apply approximates_proj in H__f. apply H__f.
-      revert Hwp2. apply dmut_wp_monotonic.
-      intros Σ3 ζ3 pc3 b3 s__sym3 H__post ι3 rel23 Hpc3.
-      apply H__post. apply (syminstance_rel_trans rel12 rel23). assumption.
-    Qed.
-
-    Lemma dmut_fresh_sound {Γ Σ ς τ} (ι : SymInstance Σ)
-          (dm : DynamicMutator Γ Γ Unit (Σ ▻ (ς,τ))) (wfdm : dmut_wf dm)
-          (sm : Lit τ -> SCMut Γ Γ unit) :
-      (forall v, box approximates (env_snoc ι _ v) dm (sm v)) ->
-      box approximates ι
-        (dmut_fresh (ς,τ) dm)
-        (scmut_demonic sm).
-    Proof.
-      intros HYP. unfold box, approximates.
-      intros * <- pc1 s1 POST Hwp Hpc.
-      apply scmut_wp_demonic. intros v.
-      specialize (HYP v (Σ1 ▻ (ς,τ)) (sub_up1 ζ1) (env_snoc ι1 (ς,τ) v)).
-      inster HYP by apply syminstance_rel_up; auto.
-      unfold approximates in HYP.
-      specialize (HYP (subst sub_wk1 pc1) (subst (sub_wk1) s1) POST).
-      rewrite ?inst_subst, ?inst_sub_wk1 in HYP. apply HYP; auto.
-      apply dmut_wp_sub_fresh in Hwp; auto using stateprop_lift_dcl.
-      revert Hwp.
-      apply dmut_wp_monotonic; cbn.
-      unfold stateprop_impl, stateprop_specialize, stateprop_lift.
-      intros ? ζ * Hpost ι0 rel10.
-      dependent elimination ζ as [@env_snoc Σ0 ζ _ t].
-      apply syminstance_rel_snoc in rel10.
-      apply Hpost. now rewrite sub_comp_wk1_tail.
-    Qed.
 
     Lemma dmut_produce_sound {Γ Σ} (asn : Assertion Σ) (ι : SymInstance Σ) :
       box approximates
@@ -1444,19 +1608,12 @@ Module Soundness
       - apply dmut_assume_formula_sound.
       - apply dmut_produce_chunk_sound.
       - apply approximates_demonic_binary.
-        + unfold dmut_bind_right.
-          eapply dmut_bind_sound.
-          apply dmut_wf_assume_formula.
-          intros. apply dmut_wf_sub, dmut_wf_produce.
-          apply dmut_assume_formula_sound.
-          intros.
-          eapply approximates_sub; eauto.
-        + eapply dmut_bind_sound.
-          apply dmut_wf_assume_formula.
-          intros. apply dmut_wf_sub, dmut_wf_produce.
-          apply dmut_assume_formula_sound.
-          intros.
-          eapply approximates_sub; eauto.
+        + unfold dmut_assume_term, scmut_assume_term.
+          apply dmut_bind_right_sound;
+            auto using dmut_assume_formula_dcl, dmut_produce_dcl, dmut_assume_formula_sound.
+        + unfold dmut_assume_term, scmut_assume_term.
+          apply dmut_bind_right_sound;
+            auto using dmut_assume_formula_dcl, dmut_produce_dcl, dmut_assume_formula_sound.
       - admit.
       - admit.
       - admit.
@@ -1464,16 +1621,13 @@ Module Soundness
       - admit.
       - admit.
       - admit.
-      - intros. apply dmut_bind_sound. admit. admit.
-        apply IHasn1. intros.
-        eapply approximates_sub; eauto.
-      - apply dmut_fresh_sound.
-        + admit.
-        + intros. apply IHasn.
+      - apply dmut_bind_right_sound; auto using dmut_produce_dcl.
+      - apply dmut_fresh_sound; auto using dmut_produce_dcl.
     Admitted.
 
-    Opaque dmut_wp.
-    Opaque scmut_wp.
+    Lemma dmut_exec_sound {Γ Σ σ} (s : Stm Γ σ) (ι : SymInstance Σ) :
+      box approximates ι (dmut_exec s) (scmut_exec s).
+    Proof. (* induction s; cbn [dmut_exec scmut_exec]. *) Admitted.
 
     Section Leftovers.
 
